exceptions

src/HOL/MicroJava/BV/Kildall.thy
@@ -1,6 +1,6 @@
-(*  Title:      HOL/BCV/Kildall.thy
+(*  Title:      HOL/MicroJava/BV/Kildall.thy
     ID:         $Id$
-    Author:     Tobias Nipkow
+    Author:     Tobias Nipkow, Gerwin Klein
     Copyright   2000 TUM
 
 Kildall's algorithm
@@ -8,84 +8,133 @@ Kildall's algorithm
 
 header "Kildall's Algorithm"
 
-theory Kildall = Typing_Framework + While_Combinator:
+theory Kildall = Typing_Framework + While_Combinator + Product:
+
+
+syntax "@lesubstep_type" :: "(nat \<times> 's) list => 's ord => (nat \<times> 's) list => bool"
+       ("(_ /<=|_| _)" [50, 0, 51] 50)
+translations
+ "x <=|r| y" == "x <=[(Product.le (op =) r)] y"
+ 
 
 constdefs
- pres_type :: "(nat => 's => 's) => nat => 's set => bool"
-"pres_type step n A == !s:A. !p<n. step p s : A"
+ pres_type :: "'s step_type => nat => 's set => bool"
+"pres_type step n A == \<forall>s\<in>A. \<forall>p<n. \<forall>(q,s')\<in>set (step p s). s' \<in> A"
 
- mono :: "'s ord => (nat => 's => 's) => nat => 's set => bool"
+ mono :: "'s ord => 's step_type => nat => 's set => bool"
 "mono r step n A ==
- !s p t. s : A & p < n & s <=_r t --> step p s <=_r step p t"
+ \<forall>s p t. s \<in> A \<and> p < n \<and> s <=_r t --> step p s <=|r| step p t"
 
 consts
- iter :: "'s binop \<Rightarrow> (nat \<Rightarrow> 's \<Rightarrow> 's) \<Rightarrow> (nat \<Rightarrow> nat list) \<Rightarrow>
+ iter :: "'s binop \<Rightarrow> 's step_type \<Rightarrow>
           's list \<Rightarrow> nat set \<Rightarrow> 's list \<times> nat set"
- propa :: "'s binop => nat list => 's => 's list => nat set => 's list * nat set"
+ propa :: "'s binop => (nat \<times> 's) list => 's list => nat set => 's list * nat set"
 
 primrec
-"propa f []     t ss w = (ss,w)"
-"propa f (q#qs) t ss w = (let u = t +_f ss!q;
-                              w' = (if u = ss!q then w else insert q w)
-                          in propa f qs t (ss[q := u]) w')"
+"propa f []      ss w = (ss,w)"
+"propa f (q'#qs) ss w = (let (q,t) = q';
+                             u = t +_f ss!q;
+                             w' = (if u = ss!q then w else insert q w)
+                         in propa f qs (ss[q := u]) w')"
 
 defs iter_def:
-"iter f step succs ss w ==
+"iter f step ss w ==
  while (%(ss,w). w \<noteq> {})
-       (%(ss,w). let p = SOME p. p : w
-                 in propa f (succs p) (step p (ss!p)) ss (w-{p}))
+       (%(ss,w). let p = SOME p. p \<in> w
+                 in propa f (step p (ss!p)) ss (w-{p}))
        (ss,w)"
 
 constdefs
- unstables ::
- "'s ord => (nat => 's => 's) => (nat => nat list) => 's list => nat set"
-"unstables r step succs ss ==
- {p. p < size ss & ~stable r step succs ss p}"
+ unstables :: "'s ord => 's step_type => 's list => nat set"
+"unstables r step ss == {p. p < size ss \<and> \<not>stable r step ss p}"
 
- kildall :: "'s ord => 's binop => (nat => 's => 's) => (nat => nat list)
-             => 's list => 's list"
-"kildall r f step succs ss == fst(iter f step succs ss (unstables r step succs ss))"
+ kildall :: "'s ord => 's binop => 's step_type => 's list => 's list"
+"kildall r f step ss == fst(iter f step ss (unstables r step ss))"
 
-consts merges :: "'s binop => 's => nat list => 's list => 's list"
+consts merges :: "'s binop => (nat \<times> 's) list => 's list => 's list"
 primrec
-"merges f s []     ss = ss"
-"merges f s (p#ps) ss = merges f s ps (ss[p := s +_f ss!p])"
+"merges f []      ss = ss"
+"merges f (p'#ps) ss = (let (p,s) = p' in merges f ps (ss[p := s +_f ss!p]))"
 
 
 lemmas [simp] = Let_def le_iff_plus_unchanged [symmetric]
 
 
+consts
+ "@plusplussub" :: "'a list => ('a => 'a => 'a) => 'a => 'a" ("(_ /++'__ _)" [65, 1000, 66] 65)
+primrec
+  "[] ++_f y = y"
+  "(x#xs) ++_f y = xs ++_f (x +_f y)"
+
+lemma nth_merges:
+  "!!ss. [| semilat (A, r, f); p < length ss; ss \<in> list n A; 
+            \<forall>(p,t)\<in>set ps. p<n \<and> t\<in>A |] ==>
+  (merges f ps ss)!p = map snd [(p',t') \<in> ps. p'=p] ++_f ss!p"
+  (is "!!ss. _ \<Longrightarrow> _ \<Longrightarrow> _ \<Longrightarrow> ?steptype ps \<Longrightarrow> ?P ss ps")
+proof (induct ps)
+  show "\<And>ss. ?P ss []" by simp
+
+  fix ss p' ps'
+  assume sl: "semilat (A, r, f)"
+  assume ss: "ss \<in> list n A"
+  assume l:  "p < length ss"
+  assume "?steptype (p'#ps')"
+  then obtain a b where
+    p': "p'=(a,b)" and ab: "a<n" "b\<in>A" and "?steptype ps'"
+    by (cases p', auto)
+  assume "\<And>ss. semilat (A,r,f) \<Longrightarrow> p < length ss \<Longrightarrow> ss \<in> list n A \<Longrightarrow> ?steptype ps' \<Longrightarrow> ?P ss ps'"
+  hence IH: "\<And>ss. ss \<in> list n A \<Longrightarrow> p < length ss \<Longrightarrow> ?P ss ps'" .
+
+  from sl ss ab
+  have "ss[a := b +_f ss!a] \<in> list n A" by (simp add: closedD)
+  moreover
+  from calculation
+  have "p < length (ss[a := b +_f ss!a])" by simp
+  ultimately
+  have "?P (ss[a := b +_f ss!a]) ps'" by (rule IH)
+  with p' l 
+  show "?P ss (p'#ps')" by simp
+qed
+
+
 lemma pres_typeD:
-  "[| pres_type step n A; s:A; p<n |] ==> step p s : A"
+  "[| pres_type step n A; s\<in>A; p<n; (q,s')\<in>set (step p s) |] ==> s' \<in> A"
   by (unfold pres_type_def, blast)
 
-lemma boundedD:
-  "[| bounded succs n; p < n; q : set(succs p) |] ==> q < n"
+lemma boundedD: 
+  "[| bounded step n; p < n; (q,t) : set (step p xs) |] ==> q < n" 
   by (unfold bounded_def, blast)
 
 lemma monoD:
-  "[| mono r step n A; p < n; s:A; s <=_r t |] ==> step p s <=_r step p t"
+  "[| mono r step n A; p < n; s\<in>A; s <=_r t |] ==> step p s <=|r| step p t"
   by (unfold mono_def, blast)
 
 (** merges **)
 
 lemma length_merges [rule_format, simp]:
-  "!ss. size(merges f t ps ss) = size ss"
+  "\<forall>ss. size(merges f ps ss) = size ss"
   by (induct_tac ps, auto)
 
-lemma merges_preserves_type [rule_format, simp]:
-  "[| semilat(A,r,f) |] ==> 
-     !xs. xs : list n A --> x : A --> (!p : set ps. p<n) 
-          --> merges f x ps xs : list n A"
-  apply (frule semilatDclosedI)
-  apply (unfold closed_def)
+
+lemma merges_preserves_type_lemma: 
+  "[| semilat(A,r,f) |] ==>
+     \<forall>xs. xs \<in> list n A --> (\<forall>(p,x) \<in> set ps. p<n \<and> x\<in>A)
+          --> merges f ps xs \<in> list n A" 
+  apply (frule semilatDclosedI) 
+  apply (unfold closed_def) 
   apply (induct_tac ps)
-  apply auto
+   apply simp
+  apply clarsimp
   done
 
-lemma merges_incr [rule_format]:
+lemma merges_preserves_type [simp]:
+  "[| semilat(A,r,f); xs \<in> list n A; \<forall>(p,x) \<in> set ps. p<n \<and> x\<in>A |]
+  ==> merges f ps xs \<in> list n A"
+  by (simp add: merges_preserves_type_lemma)
+  
+lemma merges_incr_lemma:
   "[| semilat(A,r,f) |] ==> 
-     !xs. xs : list n A --> x : A --> (!p:set ps. p<size xs) --> xs <=[r] merges f x ps xs"
+     \<forall>xs. xs \<in> list n A --> (\<forall>(p,x)\<in>set ps. p<size xs \<and> x \<in> A) --> xs <=[r] merges f ps xs"
   apply (induct_tac ps)
    apply simp
   apply simp
@@ -99,14 +148,20 @@ lemma merges_incr [rule_format]:
   apply (blast intro!: listE_set intro: closedD listE_length [THEN nth_in])
   done
 
+lemma merges_incr:
+  "[| semilat(A,r,f); xs \<in> list n A; \<forall>(p,x)\<in>set ps. p<size xs \<and> x \<in> A |] 
+  ==> xs <=[r] merges f ps xs"
+  by (simp add: merges_incr_lemma)
+
+
 lemma merges_same_conv [rule_format]:
   "[| semilat(A,r,f) |] ==> 
-     (!xs. xs : list n A --> x:A --> (!p:set ps. p<size xs) --> 
-     (merges f x ps xs = xs) = (!p:set ps. x <=_r xs!p))"
+     (\<forall>xs. xs \<in> list n A --> (\<forall>(p,x)\<in>set ps. p<size xs \<and> x\<in>A) --> 
+     (merges f ps xs = xs) = (\<forall>(p,x)\<in>set ps. x <=_r xs!p))"
   apply (induct_tac ps)
    apply simp
   apply clarsimp
-  apply (rename_tac p ps xs)
+  apply (rename_tac p x ps xs)
   apply (rule iffI)
    apply (rule context_conjI)
     apply (subgoal_tac "xs[p := x +_f xs!p] <=[r] xs")
@@ -114,8 +169,11 @@ lemma merges_same_conv [rule_format]:
     apply (erule subst, rule merges_incr)
         apply assumption
        apply (blast intro!: listE_set intro: closedD listE_length [THEN nth_in])
-     apply assumption
-    apply simp
+      apply clarify
+      apply (rule conjI)
+       apply simp
+       apply (blast dest: boundedD)
+      apply blast
    apply clarify
    apply (rotate_tac -2)
    apply (erule allE)
@@ -126,6 +184,7 @@ lemma merges_same_conv [rule_format]:
    apply (drule bspec)
     apply assumption
    apply (simp add: le_iff_plus_unchanged [THEN iffD1] list_update_same_conv [THEN iffD2])
+   apply blast
   apply clarify 
   apply (simp add: le_iff_plus_unchanged [THEN iffD1] list_update_same_conv [THEN iffD2])
   done
@@ -133,26 +192,24 @@ lemma merges_same_conv [rule_format]:
 
 lemma list_update_le_listI [rule_format]:
   "set xs <= A --> set ys <= A --> xs <=[r] ys --> p < size xs -->  
-   x <=_r ys!p --> semilat(A,r,f) --> x:A --> 
+   x <=_r ys!p --> semilat(A,r,f) --> x\<in>A --> 
    xs[p := x +_f xs!p] <=[r] ys"
   apply (unfold Listn.le_def lesub_def semilat_def)
   apply (simp add: list_all2_conv_all_nth nth_list_update)
   done
 
 lemma merges_pres_le_ub:
-  "[| semilat(A,r,f); t:A; set ts <= A; set ss <= A; 
-     !p. p:set ps --> t <=_r ts!p; 
-     !p. p:set ps --> p<size ts; 
+  "[| semilat(A,r,f); set ts <= A; set ss <= A; 
+     \<forall>(p,t)\<in>set ps. t <=_r ts!p \<and> t \<in> A \<and> p < size ts; 
      ss <=[r] ts |] 
-  ==> merges f t ps ss <=[r] ts"
+  ==> merges f ps ss <=[r] ts"
 proof -
   { fix A r f t ts ps
     have
-    "!!qs. [| semilat(A,r,f); set ts <= A; t:A; 
-       !p. p:set ps --> t <=_r ts!p; 
-       !p. p:set ps --> p<size ts |] ==> 
+    "!!qs. [| semilat(A,r,f); set ts <= A; 
+              \<forall>(p,t)\<in>set ps. t <=_r ts!p \<and> t \<in> A \<and> p < size ts |] ==> 
     set qs <= set ps  --> 
-    (!ss. set ss <= A --> ss <=[r] ts --> merges f t qs ss <=[r] ts)"
+    (\<forall>ss. set ss <= A --> ss <=[r] ts --> merges f qs ss <=[r] ts)"
     apply (induct_tac qs)
      apply simp
     apply (simp (no_asm_simp))
@@ -160,9 +217,11 @@ proof -
     apply (rotate_tac -2)
     apply simp
     apply (erule allE, erule impE, erule_tac [2] mp)
-     apply (simp (no_asm_simp) add: closedD)
+     apply (drule bspec, assumption)
+     apply (simp add: closedD)
+    apply (drule bspec, assumption)
     apply (simp add: list_update_le_listI)
-    done
+    done 
   } note this [dest]
   
   case rule_context
@@ -170,27 +229,19 @@ proof -
 qed
 
 
-lemma nth_merges [rule_format]:
-  "[| semilat (A, r, f); t:A; p < n |] ==> !ss. ss : list n A --> 
-     (!p:set ps. p<n) --> 
-     (merges f t ps ss)!p = (if p : set ps then t +_f ss!p else ss!p)"
-  apply (induct_tac "ps")
-   apply simp
-  apply (simp add: nth_list_update closedD listE_nth_in) 
-  done
-
-
 (** propa **)
 
-lemma decomp_propa [rule_format]:
-  "!ss w. (!q:set qs. q < size ss) --> 
-   propa f qs t ss w = 
-   (merges f t qs ss, {q. q:set qs & t +_f ss!q ~= ss!q} Un w)"
-  apply (induct_tac qs)
-   apply simp
+
+lemma decomp_propa:
+  "!!ss w. (\<forall>(q,t)\<in>set qs. q < size ss) \<Longrightarrow> 
+   propa f qs ss w = 
+   (merges f qs ss, {q. \<exists>t. (q,t)\<in>set qs \<and> t +_f ss!q \<noteq> ss!q} Un w)"
+  apply (induct qs)
+   apply simp   
   apply (simp (no_asm))
-  apply clarify
-  apply (rule conjI)
+  apply clarify  
+  apply simp
+  apply (rule conjI) 
    apply (simp add: nth_list_update)
    apply blast
   apply (simp add: nth_list_update)
@@ -199,57 +250,240 @@ lemma decomp_propa [rule_format]:
 
 (** iter **)
 
+lemma plusplus_closed: 
+  "\<And>y. \<lbrakk>semilat (A, r, f); set x \<subseteq> A; y \<in> A\<rbrakk> \<Longrightarrow> x ++_f y \<in> A"
+proof (induct x)
+  show "\<And>y. y \<in> A \<Longrightarrow> [] ++_f y \<in> A" by simp
+  fix y x xs
+  assume sl: "semilat (A, r, f)" and y: "y \<in> A" and xs: "set (x#xs) \<subseteq> A"
+  assume IH: "\<And>y. \<lbrakk>semilat (A, r, f); set xs \<subseteq> A; y \<in> A\<rbrakk> \<Longrightarrow> xs ++_f y \<in> A"
+  from xs obtain x: "x \<in> A" and "set xs \<subseteq> A" by simp  
+  from sl x y have "(x +_f y) \<in> A" by (simp add: closedD)
+  with sl xs have "xs ++_f (x +_f y) \<in> A" by - (rule IH)
+  thus "(x#xs) ++_f y \<in> A" by simp
+qed
+
+lemma ub2: "!!y. \<lbrakk>semilat (A, r, f); set x \<subseteq> A; y \<in> A\<rbrakk> \<Longrightarrow> y <=_r x ++_f y"
+proof (induct x)
+  show "\<And>y. semilat(A, r, f) \<Longrightarrow> y <=_r [] ++_f y" by simp 
+  
+  fix y a l
+  assume sl: "semilat (A, r, f)"
+  assume y:  "y \<in> A"
+  assume "set (a#l) \<subseteq> A"
+  then obtain a: "a \<in> A" and x: "set l \<subseteq> A" by simp 
+  assume "\<And>y. \<lbrakk>semilat (A, r, f); set l \<subseteq> A; y \<in> A\<rbrakk> \<Longrightarrow> y <=_r l ++_f y"
+  hence IH: "\<And>y. y \<in> A \<Longrightarrow> y <=_r l ++_f y" .
+
+  from sl have "order r" .. note order_trans [OF this, trans]  
+  
+  from sl a y have "y <=_r a +_f y" by (rule semilat_ub2)
+  also
+  from sl a y have "a +_f y \<in> A" by (simp add: closedD)
+  hence "(a +_f y) <=_r l ++_f (a +_f y)" by (rule IH)
+  finally
+  have "y <=_r l ++_f (a +_f y)" .
+  thus "y <=_r (a#l) ++_f y" by simp
+qed
+
+
+lemma ub1: "\<And>y. \<lbrakk>semilat (A, r, f); set ls \<subseteq> A; y \<in> A; x \<in> set ls\<rbrakk> \<Longrightarrow> x <=_r ls ++_f y"
+proof (induct ls)
+  show "\<And>y. x \<in> set [] \<Longrightarrow> x <=_r [] ++_f y" by simp
+  
+  fix y s ls
+  assume sl: "semilat (A, r, f)" 
+  hence "order r" .. note order_trans [OF this, trans]
+  assume "set (s#ls) \<subseteq> A"
+  then obtain s: "s \<in> A" and ls: "set ls \<subseteq> A" by simp
+  assume y: "y \<in> A" 
+
+  assume "\<And>y. \<lbrakk>semilat (A, r, f); set ls \<subseteq> A; y \<in> A; x \<in> set ls\<rbrakk> \<Longrightarrow> x <=_r ls ++_f y"
+  hence IH: "\<And>y. x \<in> set ls \<Longrightarrow> y \<in> A \<Longrightarrow> x <=_r ls ++_f y" .
+
+  assume "x \<in> set (s#ls)"
+  then obtain xls: "x = s \<or> x \<in> set ls" by simp
+  moreover {
+    assume xs: "x = s"
+    from sl s y have "s <=_r s +_f y" by (rule semilat_ub1)
+    also
+    from sl s y have "s +_f y \<in> A" by (simp add: closedD)
+    with sl ls have "(s +_f y) <=_r ls ++_f (s +_f y)" by (rule ub2)
+    finally 
+    have "s <=_r ls ++_f (s +_f y)" .
+    with xs have "x <=_r ls ++_f (s +_f y)" by simp
+  } 
+  moreover {
+    assume "x \<in> set ls"
+    hence "\<And>y. y \<in> A \<Longrightarrow> x <=_r ls ++_f y" by (rule IH)
+    moreover
+    from sl s y
+    have "s +_f y \<in> A" by (simp add: closedD)
+    ultimately 
+    have "x <=_r ls ++_f (s +_f y)" .
+  }
+  ultimately 
+  have "x <=_r ls ++_f (s +_f y)" by blast
+  thus "x <=_r (s#ls) ++_f y" by simp
+qed
+
+
+lemma ub1': 
+  "\<lbrakk>semilat (A, r, f); \<forall>(p,s) \<in> set S. s \<in> A; y \<in> A; (a,b) \<in> set S\<rbrakk> 
+  \<Longrightarrow> b <=_r map snd [(p', t')\<in>S. p' = a] ++_f y" 
+proof -
+  let "b <=_r ?map ++_f y" = ?thesis
+
+  assume "semilat (A, r, f)" "y \<in> A"
+  moreover
+  assume "\<forall>(p,s) \<in> set S. s \<in> A"
+  hence "set ?map \<subseteq> A" by auto
+  moreover
+  assume "(a,b) \<in> set S"
+  hence "b \<in> set ?map" by (induct S, auto)
+  ultimately
+  show ?thesis by - (rule ub1)
+qed
+    
+ 
+
+lemma plusplus_empty:  
+  "\<forall>s'. (q, s') \<in> set S \<longrightarrow> s' +_f ss ! q = ss ! q \<Longrightarrow>
+   (map snd [(p', t')\<in> S. p' = q] ++_f ss ! q) = ss ! q"
+apply (induct S)
+apply auto 
+done
+
+
 lemma stable_pres_lemma:
-  "[| semilat (A,r,f); pres_type step n A; bounded succs n; 
-     ss : list n A; p : w; ! q:w. q < n; 
-     ! q. q < n --> q ~: w --> stable r step succs ss q; q < n; 
-     q : set (succs p) --> step p (ss ! p) +_f ss ! q = ss ! q; 
-     q ~: w | q = p  |] 
-  ==> stable r step succs (merges f (step p (ss!p)) (succs p) ss) q"
+  "[| semilat (A,r,f); pres_type step n A; bounded step n; 
+     ss \<in> list n A; p \<in> w; \<forall>q\<in>w. q < n; 
+     \<forall>q. q < n \<longrightarrow> q \<notin> w \<longrightarrow> stable r step ss q; q < n; 
+     \<forall>s'. (q,s') \<in> set (step p (ss ! p)) \<longrightarrow> s' +_f ss ! q = ss ! q; 
+     q \<notin> w \<or> q = p |] 
+  ==> stable r step (merges f (step p (ss!p)) ss) q"
   apply (unfold stable_def)
-  apply (subgoal_tac "step p (ss!p) : A")
-   defer
-   apply (blast intro: listE_nth_in pres_typeD)     
+  apply (subgoal_tac "\<forall>s'. (q,s') \<in> set (step p (ss!p)) \<longrightarrow> s' : A")
+   prefer 2
+   apply clarify
+   apply (erule pres_typeD)
+    prefer 3 apply assumption
+    apply (rule listE_nth_in)
+     apply assumption
+    apply simp
+   apply simp
   apply simp
   apply clarify
-  apply (subst nth_merges)
-       apply assumption
+  apply (subst nth_merges) 
+        apply assumption
+       apply simp
+       apply (blast dest: boundedD)
       apply assumption
-     prefer 2
-     apply assumption
-    apply (blast dest: boundedD)
-   apply (blast dest: boundedD)  
-  apply (subst nth_merges)
-       apply assumption
-      apply assumption
-     prefer 2
-     apply assumption
-    apply (blast dest: boundedD)
-   apply (blast dest: boundedD)  
-  apply simp
+     apply clarify
+     apply (rule conjI)
+      apply (blast dest: boundedD)
+     apply (erule pres_typeD)
+       prefer 3 apply assumption
+      apply simp
+     apply simp 
+  apply (frule nth_merges [of _ _ _ q _ _ "step p (ss!p)"]) (* fixme: why does method subst not work?? *)
+    prefer 2 apply assumption
+   apply simp
+  apply clarify
   apply (rule conjI)
-   apply clarify
-   apply (blast intro!: semilat_ub1 semilat_ub2 listE_nth_in
-                intro: order_trans dest: boundedD)
-  apply (blast intro!: semilat_ub1 semilat_ub2 listE_nth_in
-               intro: order_trans dest: boundedD)
-  done
+   apply (blast dest: boundedD)
+  apply (erule pres_typeD)
+     prefer 3 apply assumption
+    apply simp
+   apply simp
+  apply (drule_tac P = "\<lambda>x. (a, b) \<in> set (step q x)" in subst)
+   apply assumption
 
-lemma merges_bounded_lemma [rule_format]:
-  "[| semilat (A,r,f); mono r step n A; bounded succs n; 
-     step p (ss!p) : A; ss : list n A; ts : list n A; p < n; 
-     ss <=[r] ts; ! p. p < n --> stable r step succs ts p |] 
-  ==> merges f (step p (ss!p)) (succs p) ss <=[r] ts"
+ apply (simp add: plusplus_empty)
+ apply (cases "q \<in> w")
+  apply simp
+  apply (rule ub1')
+     apply assumption
+    apply clarify
+    apply (rule pres_typeD)
+       apply assumption
+      prefer 3 apply assumption
+     apply (blast intro: listE_nth_in dest: boundedD)
+    apply (blast intro: pres_typeD dest: boundedD)
+   apply (blast intro: listE_nth_in dest: boundedD)
+  apply assumption
+
+ apply simp
+ apply (erule allE, erule impE, assumption, erule impE, assumption)
+ apply (rule order_trans)
+   apply simp
+  defer
+ apply (rule ub2)
+    apply assumption
+   apply simp
+   apply clarify
+   apply simp
+   apply (rule pres_typeD)
+      apply assumption
+     prefer 3 apply assumption
+    apply (blast intro: listE_nth_in dest: boundedD)
+   apply (blast intro: pres_typeD dest: boundedD)
+  apply (blast intro: listE_nth_in dest: boundedD)
+ apply blast
+ done
+ 
+  
+lemma lesub_step_type:
+  "!!b x y. a <=|r| b \<Longrightarrow> (x,y) \<in> set a \<Longrightarrow> \<exists>y'. (x, y') \<in> set b \<and> y <=_r y'"
+apply (induct a)
+ apply simp
+apply simp
+apply (case_tac b)
+ apply simp
+apply simp
+apply (erule disjE)
+ apply clarify
+ apply (simp add: lesub_def)
+ apply blast   
+apply clarify
+apply blast
+done
+
+
+lemma merges_bounded_lemma:
+  "[| semilat (A,r,f); mono r step n A; bounded step n; 
+     \<forall>(p',s') \<in> set (step p (ss!p)). s' \<in> A; ss \<in> list n A; ts \<in> list n A; p < n; 
+     ss <=[r] ts; ! p. p < n --> stable r step ts p |] 
+  ==> merges f (step p (ss!p)) ss <=[r] ts"
   apply (unfold stable_def)
-  apply (blast intro!: listE_set monoD listE_nth_in le_listD less_lengthI
-               intro: merges_pres_le_ub order_trans
-               dest: pres_typeD boundedD)
+  apply (rule merges_pres_le_ub)
+      apply assumption
+     apply simp
+    apply simp
+   prefer 2 apply assumption
+
+  apply clarsimp
+  apply (drule boundedD, assumption+)
+  apply (erule allE, erule impE, assumption)
+  apply (drule bspec, assumption)
+  apply simp
+
+  apply (drule monoD [of _ _ _ _ p "ss!p"  "ts!p"])
+     apply assumption
+    apply simp
+   apply (simp add: le_listD)
+  
+  apply (drule lesub_step_type, assumption) 
+  apply clarify
+  apply (drule bspec, assumption)
+  apply simp
+  apply (blast intro: order_trans)
   done
 
 lemma termination_lemma:  
-  "[| semilat(A,r,f); ss : list n A; t:A; ! q:set qs. q < n; p:w |] ==> 
-      ss <[r] merges f t qs ss | 
-  merges f t qs ss = ss & {q. q:set qs & t +_f ss!q ~= ss!q} Un (w-{p}) < w"
+  "[| semilat(A,r,f); ss \<in> list n A; \<forall>(q,t)\<in>set qs. q<n \<and> t\<in>A; p\<in>w |] ==> 
+      ss <[r] merges f qs ss \<or> 
+  merges f qs ss = ss \<and> {q. \<exists>t. (q,t)\<in>set qs \<and> t +_f ss!q \<noteq> ss!q} Un (w-{p}) < w"
   apply (unfold lesssub_def)
   apply (simp (no_asm_simp) add: merges_incr)
   apply (rule impI)
@@ -257,88 +491,126 @@ lemma termination_lemma:
   apply assumption+
     defer
     apply (rule sym, assumption)
-   apply (simp cong add: conj_cong add: le_iff_plus_unchanged [symmetric])
+   defer apply simp
+   apply (subgoal_tac "\<forall>q t. \<not>((q, t) \<in> set qs \<and> t +_f ss ! q \<noteq> ss ! q)")
    apply (blast intro!: psubsetI elim: equalityE)
-  apply simp
-  done
+   apply clarsimp
+   apply (drule bspec, assumption) 
+   apply (drule bspec, assumption)
+   apply clarsimp
+  done 
 
 lemma iter_properties[rule_format]:
   "\<lbrakk> semilat(A,r,f); acc r ; pres_type step n A; mono r step n A;
-     bounded succs n; \<forall>p\<in>w0. p < n; ss0 \<in> list n A;
-     \<forall>p<n. p \<notin> w0 \<longrightarrow> stable r step succs ss0 p \<rbrakk> \<Longrightarrow>
-   iter f step succs ss0 w0 = (ss',w')
+     bounded step n; \<forall>p\<in>w0. p < n; ss0 \<in> list n A;
+     \<forall>p<n. p \<notin> w0 \<longrightarrow> stable r step ss0 p \<rbrakk> \<Longrightarrow>
+   iter f step ss0 w0 = (ss',w')
    \<longrightarrow>
-   ss' \<in> list n A \<and> stables r step succs ss' \<and> ss0 <=[r] ss' \<and>
-   (\<forall>ts\<in>list n A. ss0 <=[r] ts \<and> stables r step succs ts \<longrightarrow> ss' <=[r] ts)"
+   ss' \<in> list n A \<and> stables r step ss' \<and> ss0 <=[r] ss' \<and>
+   (\<forall>ts\<in>list n A. ss0 <=[r] ts \<and> stables r step ts \<longrightarrow> ss' <=[r] ts)"
 apply (unfold iter_def stables_def)
 apply (rule_tac P = "%(ss,w).
- ss \<in> list n A \<and> (\<forall>p<n. p \<notin> w \<longrightarrow> stable r step succs ss p) \<and> ss0 <=[r] ss \<and>
- (\<forall>ts\<in>list n A. ss0 <=[r] ts \<and> stables r step succs ts \<longrightarrow> ss <=[r] ts) \<and>
+ ss \<in> list n A \<and> (\<forall>p<n. p \<notin> w \<longrightarrow> stable r step ss p) \<and> ss0 <=[r] ss \<and>
+ (\<forall>ts\<in>list n A. ss0 <=[r] ts \<and> stables r step ts \<longrightarrow> ss <=[r] ts) \<and>
  (\<forall>p\<in>w. p < n)" and
  r = "{(ss',ss) . ss <[r] ss'} <*lex*> finite_psubset"
        in while_rule)
 
-(* Invariant holds initially: *)
-apply (simp add:stables_def)
-(* Invariant is preserved: *)
+-- "Invariant holds initially:"
+apply (simp add:stables_def) 
+
+-- "Invariant is preserved:"
 apply(simp add: stables_def split_paired_all)
 apply(rename_tac ss w)
 apply(subgoal_tac "(SOME p. p \<in> w) \<in> w")
  prefer 2; apply (fast intro: someI)
-apply(subgoal_tac "step (SOME p. p \<in> w) (ss ! (SOME p. p \<in> w)) \<in> A")
- prefer 2; apply (blast intro: pres_typeD listE_nth_in dest: boundedD);
-  apply (subgoal_tac "\<forall>q\<in>set(succs (SOME p. p \<in> w)). q < size ss")
- prefer 2;  apply(clarsimp, blast dest!: boundedD)
+apply(subgoal_tac "\<forall>(q,t) \<in> set (step (SOME p. p \<in> w) (ss ! (SOME p. p \<in> w))). q < length ss \<and> t \<in> A")
+ prefer 2
+ apply clarify
+ apply (rule conjI)
+  apply(clarsimp, blast dest!: boundedD)
+ apply (erule pres_typeD)
+  prefer 3
+  apply assumption
+  apply (erule listE_nth_in)
+  apply blast
+ apply blast
 apply (subst decomp_propa)
  apply blast
 apply simp
 apply (rule conjI)
- apply (blast intro: merges_preserves_type dest: boundedD);
-apply (rule conjI)
+ apply (erule merges_preserves_type)
+ apply blast 
+ apply clarify
+ apply (rule conjI)
+  apply(clarsimp, blast dest!: boundedD)
+ apply (erule pres_typeD)
+  prefer 3
+  apply assumption
+  apply (erule listE_nth_in)
+  apply blast
+ apply blast
+apply (rule conjI) 
+ apply clarify 
  apply (blast intro!: stable_pres_lemma)
-apply (rule conjI)
+apply (rule conjI) 
  apply (blast intro!: merges_incr intro: le_list_trans)
 apply (rule conjI)
  apply clarsimp
- apply (best intro!: merges_bounded_lemma)
+ apply (blast intro!: merges_bounded_lemma)
 apply (blast dest!: boundedD)
 
-(* Postcondition holds upon termination: *)
-apply(clarsimp simp add: stables_def split_paired_all)
 
-(* Well-foundedness of the termination relation: *)
+-- "Postcondition holds upon termination:"
+apply(clarsimp simp add: stables_def split_paired_all) 
+
+-- "Well-foundedness of the termination relation:"
 apply (rule wf_lex_prod)
  apply (drule (1) semilatDorderI [THEN acc_le_listI])
  apply (simp only: acc_def lesssub_def)
-apply (rule wf_finite_psubset)
+apply (rule wf_finite_psubset) 
 
-(* Loop decreases along termination relation: *)
+-- "Loop decreases along termination relation:"
 apply(simp add: stables_def split_paired_all)
 apply(rename_tac ss w)
 apply(subgoal_tac "(SOME p. p \<in> w) \<in> w")
  prefer 2; apply (fast intro: someI)
-apply(subgoal_tac "step (SOME p. p \<in> w) (ss ! (SOME p. p \<in> w)) \<in> A")
- prefer 2; apply (blast intro: pres_typeD listE_nth_in dest: boundedD);
-  apply (subgoal_tac "\<forall>q\<in>set(succs (SOME p. p \<in> w)). q < n")
- prefer 2;  apply(clarsimp, blast dest!: boundedD)
+apply(subgoal_tac "\<forall>(q,t) \<in> set (step (SOME p. p \<in> w) (ss ! (SOME p. p \<in> w))). q < length ss \<and> t \<in> A")
+ prefer 2
+ apply clarify
+ apply (rule conjI)
+  apply(clarsimp, blast dest!: boundedD)
+ apply (erule pres_typeD)
+  prefer 3
+  apply assumption
+  apply (erule listE_nth_in)
+  apply blast
+ apply blast
 apply (subst decomp_propa)
- apply clarsimp
-apply clarify
+ apply blast
+apply clarify 
 apply (simp del: listE_length
-    add: lex_prod_def finite_psubset_def decomp_propa termination_lemma
+    add: lex_prod_def finite_psubset_def 
          bounded_nat_set_is_finite)
-done
+apply (rule termination_lemma)
+apply assumption+
+defer
+apply assumption
+apply clarsimp
+apply (blast dest!: boundedD)
+done   
+
 
 lemma kildall_properties:
   "\<lbrakk> semilat(A,r,f); acc r; pres_type step n A; mono r step n A;
-     bounded succs n; ss0 \<in> list n A \<rbrakk> \<Longrightarrow>
-  kildall r f step succs ss0 : list n A \<and>
-  stables r step succs (kildall r f step succs ss0) \<and>
-  ss0 <=[r] kildall r f step succs ss0 \<and>
-  (\<forall>ts\<in>list n A. ss0 <=[r] ts \<and> stables r step succs ts \<longrightarrow>
-                 kildall r f step succs ss0 <=[r] ts)";
+     bounded step n; ss0 \<in> list n A \<rbrakk> \<Longrightarrow>
+  kildall r f step ss0 \<in> list n A \<and>
+  stables r step (kildall r f step ss0) \<and>
+  ss0 <=[r] kildall r f step ss0 \<and>
+  (\<forall>ts\<in>list n A. ss0 <=[r] ts \<and> stables r step ts \<longrightarrow>
+                 kildall r f step ss0 <=[r] ts)"
 apply (unfold kildall_def)
-apply(case_tac "iter f step succs ss0 (unstables r step succs ss0)")
+apply(case_tac "iter f step ss0 (unstables r step ss0)")
 apply(simp)
 apply (rule iter_properties)
 apply (simp_all add: unstables_def stable_def)
@@ -346,23 +618,23 @@ done
 
 lemma is_bcv_kildall:
   "[| semilat(A,r,f); acc r; top r T; 
-      pres_type step n A; bounded succs n; 
+      pres_type step n A; bounded step n; 
       mono r step n A |]
-  ==> is_bcv r T step succs n A (kildall r f step succs)"
+  ==> is_bcv r T step n A (kildall r f step)"
 apply(unfold is_bcv_def wt_step_def)
 apply(insert kildall_properties[of A])
 apply(simp add:stables_def)
 apply clarify
-apply(subgoal_tac "kildall r f step succs ss : list n A")
+apply(subgoal_tac "kildall r f step ss \<in> list n A")
  prefer 2 apply (simp(no_asm_simp))
 apply (rule iffI)
- apply (rule_tac x = "kildall r f step succs ss" in bexI)
+ apply (rule_tac x = "kildall r f step ss" in bexI) 
   apply (rule conjI)
    apply blast
   apply (simp  (no_asm_simp))
  apply assumption
 apply clarify
-apply(subgoal_tac "kildall r f step succs ss!p <=_r ts!p")
+apply(subgoal_tac "kildall r f step ss!p <=_r ts!p")
  apply simp
 apply (blast intro!: le_listD less_lengthI)
 done
