src/HOL/MicroJava/BV/BVSpec.thy
@@ -1,63 +1,60 @@
 (*  Title:      HOL/MicroJava/BV/BVSpec.thy
     ID:         $Id$
-    Author:     Cornelia Pusch
+    Author:     Cornelia Pusch, Gerwin Klein
     Copyright   1999 Technische Universitaet Muenchen
 
 *)
 
 header "The Bytecode Verifier"
 
-theory BVSpec = Step:
+theory BVSpec = Effect:
+
+text {*
+  This theory contains a specification of the BV. The specification
+  describes correct typings of method bodies; it corresponds 
+  to type \emph{checking}.
+*}
 
 constdefs
-wt_instr :: "[instr,jvm_prog,ty,method_type,nat,p_count,p_count] => bool"
-"wt_instr i G rT phi mxs max_pc pc == 
-    app i G mxs rT (phi!pc) \<and>
-   (\<forall> pc' \<in> set (succs i pc). pc' < max_pc \<and> (G \<turnstile> step i G (phi!pc) <=' phi!pc'))"
+  wt_instr :: "[instr,jvm_prog,ty,method_type,nat,p_count,
+                exception_table,p_count] => bool"
+  "wt_instr i G rT phi mxs max_pc et pc == 
+  app i G mxs rT pc et (phi!pc) \<and>
+  (\<forall>(pc',s') \<in> set (eff i G pc et (phi!pc)). pc' < max_pc \<and> G \<turnstile> s' <=' phi!pc')"
 
-wt_start :: "[jvm_prog,cname,ty list,nat,method_type] => bool"
-"wt_start G C pTs mxl phi == 
-    G \<turnstile> Some ([],(OK (Class C))#((map OK pTs))@(replicate mxl Err)) <=' phi!0"
+  wt_start :: "[jvm_prog,cname,ty list,nat,method_type] => bool"
+  "wt_start G C pTs mxl phi == 
+  G \<turnstile> Some ([],(OK (Class C))#((map OK pTs))@(replicate mxl Err)) <=' phi!0"
 
+  wt_method :: "[jvm_prog,cname,ty list,ty,nat,nat,instr list,
+                 exception_table,method_type] => bool"
+  "wt_method G C pTs rT mxs mxl ins et phi ==
+  let max_pc = length ins in
+  0 < max_pc \<and> wt_start G C pTs mxl phi \<and> 
+  (\<forall>pc. pc<max_pc --> wt_instr (ins ! pc) G rT phi mxs max_pc et pc)"
 
-wt_method :: "[jvm_prog,cname,ty list,ty,nat,nat,instr list,method_type] => bool"
-"wt_method G C pTs rT mxs mxl ins phi ==
-	let max_pc = length ins
-        in
-	0 < max_pc \<and> wt_start G C pTs mxl phi \<and> 
-	(\<forall>pc. pc<max_pc --> wt_instr (ins ! pc) G rT phi mxs max_pc pc)"
-
-wt_jvm_prog :: "[jvm_prog,prog_type] => bool"
-"wt_jvm_prog G phi ==
-   wf_prog (\<lambda>G C (sig,rT,(maxs,maxl,b)).
-              wt_method G C (snd sig) rT maxs maxl b (phi C sig)) G"
-
+  wt_jvm_prog :: "[jvm_prog,prog_type] => bool"
+  "wt_jvm_prog G phi ==
+  wf_prog (\<lambda>G C (sig,rT,(maxs,maxl,b,et)).
+           wt_method G C (snd sig) rT maxs maxl b et (phi C sig)) G"
 
 
 lemma wt_jvm_progD:
-"wt_jvm_prog G phi ==> (\<exists>wt. wf_prog wt G)"
-by (unfold wt_jvm_prog_def, blast)
+  "wt_jvm_prog G phi ==> (\<exists>wt. wf_prog wt G)"
+  by (unfold wt_jvm_prog_def, blast)
 
 lemma wt_jvm_prog_impl_wt_instr:
-"[| wt_jvm_prog G phi; is_class G C;
-    method (G,C) sig = Some (C,rT,maxs,maxl,ins); pc < length ins |] 
- ==> wt_instr (ins!pc) G rT (phi C sig) maxs (length ins) pc";
-by (unfold wt_jvm_prog_def, drule method_wf_mdecl, 
-    simp, simp, simp add: wf_mdecl_def wt_method_def)
+  "[| wt_jvm_prog G phi; is_class G C;
+      method (G,C) sig = Some (C,rT,maxs,maxl,ins,et); pc < length ins |] 
+  ==> wt_instr (ins!pc) G rT (phi C sig) maxs (length ins) et pc";
+  by (unfold wt_jvm_prog_def, drule method_wf_mdecl, 
+      simp, simp, simp add: wf_mdecl_def wt_method_def)
 
 lemma wt_jvm_prog_impl_wt_start:
-"[| wt_jvm_prog G phi; is_class G C;
-    method (G,C) sig = Some (C,rT,maxs,maxl,ins) |] ==> 
- 0 < (length ins) \<and> wt_start G C (snd sig) maxl (phi C sig)"
-by (unfold wt_jvm_prog_def, drule method_wf_mdecl, 
-    simp, simp, simp add: wf_mdecl_def wt_method_def)
-
-text {* for most instructions wt\_instr collapses: *}
-lemma  
-"succs i pc = [pc+1] ==> wt_instr i G rT phi mxs max_pc pc = 
- (app i G mxs rT (phi!pc) \<and> pc+1 < max_pc \<and> (G \<turnstile> step i G (phi!pc) <=' phi!(pc+1)))"
-by (simp add: wt_instr_def) 
+  "[| wt_jvm_prog G phi; is_class G C;
+      method (G,C) sig = Some (C,rT,maxs,maxl,ins,et) |] ==> 
+  0 < (length ins) \<and> wt_start G C (snd sig) maxl (phi C sig)"
+  by (unfold wt_jvm_prog_def, drule method_wf_mdecl, 
+      simp, simp, simp add: wf_mdecl_def wt_method_def)
 
 end
-
-
