src/HOL/MicroJava/BV/BVSpecTypeSafe.thy
@@ -1,42 +1,594 @@
 (*  Title:      HOL/MicroJava/BV/BVSpecTypeSafe.thy
     ID:         $Id$
-    Author:     Cornelia Pusch
+    Author:     Cornelia Pusch, Gerwin Klein
     Copyright   1999 Technische Universitaet Muenchen
-Proof that the specification of the bytecode verifier only admits type safe
-programs.
 *)
 
 header "BV Type Safety Proof"
 
 theory BVSpecTypeSafe = Correct:
 
+text {*
+  This theory contains proof that the specification of the bytecode
+  verifier only admits type safe programs.  
+*}
+
+section {* Preliminaries *}
+
+text {*
+  Simp and intro setup for the type safety proof:
+*}
 lemmas defs1 = sup_state_conv correct_state_def correct_frame_def 
-               wt_instr_def step_def
+               wt_instr_def eff_def norm_eff_def 
 
 lemmas widen_rules[intro] = approx_val_widen approx_loc_widen approx_stk_widen
 
 lemmas [simp del] = split_paired_All
 
+
+text {*
+  If we have a welltyped program and a conforming state, we
+  can directly infer that the current instruction is well typed:
+*}
 lemma wt_jvm_prog_impl_wt_instr_cor:
-  "[| wt_jvm_prog G phi; method (G,C) sig = Some (C,rT,maxs,maxl,ins); 
+  "[| wt_jvm_prog G phi; method (G,C) sig = Some (C,rT,maxs,maxl,ins,et); 
       G,phi \<turnstile>JVM (None, hp, (stk,loc,C,sig,pc)#frs)\<surd> |] 
-  ==> wt_instr (ins!pc) G rT (phi C sig) maxs (length ins) pc"
+  ==> wt_instr (ins!pc) G rT (phi C sig) maxs (length ins) et pc"
 apply (unfold correct_state_def Let_def correct_frame_def)
 apply simp
 apply (blast intro: wt_jvm_prog_impl_wt_instr)
 done
 
+
+section {* Exception Handling *}
+
+text {*
+  Exceptions don't touch anything except the stack:
+*}
+lemma exec_instr_xcpt:
+  "(fst (exec_instr i G hp stk vars Cl sig pc frs) = Some xcp)
+  = (\<exists>stk'. exec_instr i G hp stk vars Cl sig pc frs = 
+            (Some xcp, hp, (stk', vars, Cl, sig, pc)#frs))"
+  by (cases i, auto simp add: split_beta split: split_if_asm)
+
+
+text {*
+  Relates @{text match_any} from the Bytecode Verifier with 
+  @{text match_exception_table} from the operational semantics:
+*}
+lemma in_match_any:
+  "match_exception_table G xcpt pc et = Some pc' ==> 
+  \<exists>C. C \<in> set (match_any G pc et) \<and> G \<turnstile> xcpt \<preceq>C C \<and> 
+      match_exception_table G C pc et = Some pc'"
+  (is "PROP ?P et" is "?match et ==> ?match_any et")
+proof (induct et)  
+  show "PROP ?P []" 
+    by simp
+
+  fix e es
+  assume IH: "PROP ?P es"
+  assume match: "?match (e#es)"
+
+  obtain start_pc end_pc handler_pc catch_type where
+    e [simp]: "e = (start_pc, end_pc, handler_pc, catch_type)"
+    by (cases e) 
+
+  from IH match
+  show "?match_any (e#es)" 
+  proof (cases "match_exception_entry G xcpt pc e")
+    case False
+    with match
+    have "match_exception_table G xcpt pc es = Some pc'" by simp
+    with IH
+    obtain C where
+      set: "C \<in> set (match_any G pc es)" and
+      C:   "G \<turnstile> xcpt \<preceq>C C" and
+      m:   "match_exception_table G C pc es = Some pc'" by blast
+
+    from set
+    have "C \<in> set (match_any G pc (e#es))" by simp
+    moreover
+    from False C
+    have "\<not> match_exception_entry G C pc e"
+      by - (erule contrapos_nn, 
+            auto simp add: match_exception_entry_def elim: rtrancl_trans)
+    with m
+    have "match_exception_table G C pc (e#es) = Some pc'" by simp
+    moreover note C
+    ultimately
+    show ?thesis by blast
+  next
+    case True with match
+    have "match_exception_entry G catch_type pc e"
+      by (simp add: match_exception_entry_def)
+    moreover
+    from True match
+    obtain 
+      "start_pc \<le> pc" 
+      "pc < end_pc" 
+      "G \<turnstile> xcpt \<preceq>C catch_type" 
+      "handler_pc = pc'" 
+      by (simp add: match_exception_entry_def)
+    ultimately
+    show ?thesis by auto
+  qed
+qed
+
+text {*
+  We can prove separately that the recursive search for exception
+  handlers (@{text find_handler}) in the frame stack results in 
+  a conforming state (if there was no matching exception handler 
+  in the current frame). We require that the exception is a valid
+  heap address, and that the state before the exception occured
+  conforms. 
+*}
+lemma uncaught_xcpt_correct:
+  "!!f. [| wt_jvm_prog G phi; xcp = Addr adr; hp adr = Some T;
+      G,phi \<turnstile>JVM (None, hp, f#frs)\<surd> |]
+  ==> G,phi \<turnstile>JVM (find_handler G (Some xcp) hp frs)\<surd>" 
+  (is "!!f. [| ?wt; ?adr; ?hp; ?correct (None, hp, f#frs) |] ==> ?correct (?find frs)")
+proof (induct frs) 
+  -- "the base case is trivial, as it should be"
+  show "?correct (?find [])" by (simp add: correct_state_def)
+
+  -- "we will need both forms @{text wt_jvm_prog} and @{text wf_prog} later"
+  assume wt: ?wt 
+  then obtain mb where wf: "wf_prog mb G" by (simp add: wt_jvm_prog_def)
+
+  -- "these two don't change in the induction:"
+  assume adr: ?adr
+  assume hp: ?hp
+  
+  -- "the assumption for the cons case:"
+  fix f f' frs' 
+  assume cr: "?correct (None, hp, f#f'#frs')" 
+
+  -- "the induction hypothesis as produced by Isabelle, immediatly simplified
+    with the fixed assumptions above"
+  assume "\<And>f. [| ?wt; ?adr; ?hp; ?correct (None, hp, f#frs') |] ==> ?correct (?find frs')"  
+  with wt adr hp 
+  have IH: "\<And>f. ?correct (None, hp, f#frs') ==> ?correct (?find frs')" by blast
+
+  from cr
+  have cr': "?correct (None, hp, f'#frs')" by (auto simp add: correct_state_def)
+    
+  obtain stk loc C sig pc where f' [simp]: "f' = (stk,loc,C,sig,pc)"
+    by (cases f') 
+
+  from cr 
+  obtain rT maxs maxl ins et where
+    meth: "method (G,C) sig = Some (C,rT,maxs,maxl,ins,et)"
+    by (simp add: correct_state_def, blast)
+
+  hence [simp]: "ex_table_of (snd (snd (the (method (G, C) sig)))) = et"
+    by simp
+
+  show "?correct (?find (f'#frs'))" 
+  proof (cases "match_exception_table G (cname_of hp xcp) pc et")
+    case None
+    with cr' IH 
+    show ?thesis by simp
+  next
+    fix handler_pc 
+    assume match: "match_exception_table G (cname_of hp xcp) pc et = Some handler_pc"
+    (is "?match (cname_of hp xcp) = _")
+
+    from wt meth cr' [simplified]
+    have wti: "wt_instr (ins!pc) G rT (phi C sig) maxs (length ins) et pc" 
+      by (rule wt_jvm_prog_impl_wt_instr_cor)
+
+    from cr meth
+    obtain C' mn pts ST LT where
+      ins: "ins!pc = Invoke C' mn pts" (is "_ = ?i") and
+      phi: "phi C sig ! pc = Some (ST, LT)"
+      by (simp add: correct_state_def) blast    
+
+    from match
+    obtain D where
+      in_any: "D \<in> set (match_any G pc et)" and
+      D:      "G \<turnstile> cname_of hp xcp \<preceq>C D" and
+      match': "?match D = Some handler_pc"
+      by (blast dest: in_match_any)
+
+    from ins wti phi have 
+      "\<forall>D\<in>set (match_any G pc et). the (?match D) < length ins \<and> 
+      G \<turnstile> Some ([Class D], LT) <=' phi C sig!the (?match D)"
+      by (simp add: wt_instr_def eff_def xcpt_eff_def)      
+    with in_any match' obtain
+      pc: "handler_pc < length ins" 
+      "G \<turnstile> Some ([Class D], LT) <=' phi C sig ! handler_pc"
+      by auto
+    then obtain ST' LT' where
+      phi': "phi C sig ! handler_pc = Some (ST',LT')" and
+      less: "G \<turnstile> ([Class D], LT) <=s (ST',LT')"
+      by auto    
+    
+    from cr' phi meth f'
+    have "correct_frame G hp (ST, LT) maxl ins f'"
+      by (unfold correct_state_def) auto
+    then obtain
+     len: "length loc = 1+length (snd sig)+maxl" and
+     loc: "approx_loc G hp loc LT"
+      by (unfold correct_frame_def) auto
+
+    let ?f = "([xcp], loc, C, sig, handler_pc)"
+    have "correct_frame G hp (ST', LT') maxl ins ?f" 
+    proof -
+      from wf less loc
+      have "approx_loc G hp loc LT'" by (simp add: sup_state_conv) blast
+      moreover
+      from D adr hp
+      have "G,hp \<turnstile> xcp ::\<preceq> Class D" by (simp add: conf_def obj_ty_def)
+      with wf less loc
+      have "approx_stk G hp [xcp] ST'"
+        by (auto simp add: sup_state_conv approx_stk_def approx_val_def 
+                 elim: conf_widen split: Err.split)
+      moreover
+      note len pc
+      ultimately
+      show ?thesis by (simp add: correct_frame_def)
+    qed
+
+    with cr' match phi' meth  
+    show ?thesis by (unfold correct_state_def) auto
+  qed
+qed
+
+
+text {*
+  The requirement of lemma @{text uncaught_xcpt_correct} (that
+  the exception is a valid reference on the heap) is always met
+  for welltyped instructions and conformant states:
+*}
+lemma exec_instr_xcpt_hp:
+  "[|  fst (exec_instr (ins!pc) G hp stk vars Cl sig pc frs) = Some xcp;
+       wt_instr (ins!pc) G rT (phi C sig) maxs (length ins) et pc;
+       G,phi \<turnstile>JVM (None, hp, (stk,loc,C,sig,pc)#frs)\<surd> |]
+  ==> \<exists>adr T. xcp = Addr adr \<and> hp adr = Some T" 
+  (is "[| ?xcpt; ?wt; ?correct |] ==> ?thesis")
+proof -
+  note [simp] = system_xcpt_allocated split_beta raise_system_xcpt_def
+  note [split] = split_if_asm option.split_asm 
+  
+  assume wt: ?wt ?correct
+
+  assume xcpt: ?xcpt
+  thus ?thesis 
+  proof (cases "ins!pc")
+    case New with xcpt
+    show ?thesis by (auto dest: new_Addr_OutOfMemory)
+  next
+    case Throw with xcpt wt
+    show ?thesis
+      by (auto simp add: wt_instr_def correct_state_def correct_frame_def 
+               dest: non_npD)
+  qed auto
+qed
+
+
+text {*
+  Finally we can state that, whenever an exception occurs, the
+  resulting next state always conforms:
+*}
+lemma xcpt_correct:
+  "[| wt_jvm_prog G phi;
+      method (G,C) sig = Some (C,rT,maxs,maxl,ins,et); 
+      wt_instr (ins!pc) G rT (phi C sig) maxs (length ins) et pc; 
+      fst (exec_instr (ins!pc) G hp stk loc C sig pc frs) = Some xcp; 
+      Some state' = exec (G, None, hp, (stk,loc,C,sig,pc)#frs); 
+      G,phi \<turnstile>JVM (None, hp, (stk,loc,C,sig,pc)#frs)\<surd> |] 
+  ==> G,phi \<turnstile>JVM state'\<surd>"
+proof -
+  assume wtp: "wt_jvm_prog G phi"
+  assume meth: "method (G,C) sig = Some (C,rT,maxs,maxl,ins,et)"
+  assume wt: "wt_instr (ins!pc) G rT (phi C sig) maxs (length ins) et pc"
+  assume xp: "fst (exec_instr (ins!pc) G hp stk loc C sig pc frs) = Some xcp"
+  assume s': "Some state' = exec (G, None, hp, (stk,loc,C,sig,pc)#frs)"
+  assume correct: "G,phi \<turnstile>JVM (None, hp, (stk,loc,C,sig,pc)#frs)\<surd>"
+
+  from wtp obtain wfmb where wf: "wf_prog wfmb G" by (simp add: wt_jvm_prog_def)
+
+  note xp' = meth s' xp
+
+  note wtp
+  moreover
+  from xp wt correct
+  obtain adr T where
+    adr: "xcp = Addr adr" "hp adr = Some T"
+    by (blast dest: exec_instr_xcpt_hp)
+  moreover
+  note correct
+  ultimately
+  have "G,phi \<turnstile>JVM find_handler G (Some xcp) hp frs \<surd>" by (rule uncaught_xcpt_correct)
+  with xp'
+  have "match_exception_table G (cname_of hp xcp) pc et = None \<Longrightarrow> ?thesis" 
+    (is "?m (cname_of hp xcp) = _ \<Longrightarrow> _" is "?match = _ \<Longrightarrow> _")
+    by (clarsimp simp add: exec_instr_xcpt split_beta)
+  moreover
+  { fix handler
+    assume some_handler: "?match = Some handler"
+    
+    from correct meth
+    obtain ST LT where
+      hp_ok:  "G \<turnstile>h hp \<surd>" and
+      class:  "is_class G C" and
+      phi_pc: "phi C sig ! pc = Some (ST, LT)" and
+      frame:  "correct_frame G hp (ST, LT) maxl ins (stk, loc, C, sig, pc)" and
+      frames: "correct_frames G hp phi rT sig frs"
+      by (unfold correct_state_def) auto
+
+    from frame obtain 
+      stk: "approx_stk G hp stk ST" and
+      loc: "approx_loc G hp loc LT" and
+      pc:  "pc < length ins" and
+      len: "length loc = 1+length (snd sig)+maxl"
+      by (unfold correct_frame_def) auto
+    
+    from wt obtain
+      eff: "\<forall>(pc', s')\<in>set (xcpt_eff (ins!pc) G pc (phi C sig!pc) et).
+             pc' < length ins \<and> G \<turnstile> s' <=' phi C sig!pc'"
+      by (simp add: wt_instr_def eff_def)
+    
+    from some_handler xp'
+    have state': 
+      "state' = (None, hp, ([xcp], loc, C, sig, handler)#frs)"
+      by (cases "ins!pc", auto simp add: raise_system_xcpt_def split_beta 
+                               split: split_if_asm) (* takes long! *)
+
+    let ?f' = "([xcp], loc, C, sig, handler)"
+    from eff
+    obtain ST' LT' where
+      phi_pc': "phi C sig ! handler = Some (ST', LT')" and
+      frame': "correct_frame G hp (ST',LT') maxl ins ?f'" 
+    proof (cases "ins!pc")
+      case Return -- "can't generate exceptions:"
+      with xp' have False by (simp add: split_beta split: split_if_asm)
+      thus ?thesis ..
+    next
+      case New
+      with some_handler xp'
+      have xcp: "xcp = Addr (XcptRef OutOfMemory)"
+        by (simp add: raise_system_xcpt_def split_beta new_Addr_OutOfMemory)
+      hence "cname_of hp xcp = Xcpt OutOfMemory" 
+        by (simp add: system_xcpt_allocated)
+      with New some_handler phi_pc eff 
+      obtain ST' LT' where
+        phi': "phi C sig ! handler = Some (ST', LT')" and
+        less: "G \<turnstile> ([Class (Xcpt OutOfMemory)], LT) <=s (ST', LT')" and
+        pc':  "handler < length ins"
+        by (simp add: xcpt_eff_def) blast
+      note phi'
+      moreover
+      { from xcp
+        have "G,hp \<turnstile> xcp ::\<preceq> Class (Xcpt OutOfMemory)"
+          by (simp add: conf_def obj_ty_def system_xcpt_allocated)
+        moreover
+        from wf less loc
+        have "approx_loc G hp loc LT'"
+          by (simp add: sup_state_conv) blast        
+        moreover
+        note wf less pc' len 
+        ultimately
+        have "correct_frame G hp (ST',LT') maxl ins ?f'"
+          by (unfold correct_frame_def) (auto simp add: sup_state_conv 
+              approx_stk_def approx_val_def split: err.split elim: conf_widen)
+      }
+      ultimately
+      show ?thesis by (rule that)
+    next 
+      case Getfield
+      with some_handler xp'
+      have xcp: "xcp = Addr (XcptRef NullPointer)"
+        by (simp add: raise_system_xcpt_def split_beta split: split_if_asm)
+      hence "cname_of hp xcp = Xcpt NullPointer" 
+        by (simp add: system_xcpt_allocated)
+      with Getfield some_handler phi_pc eff 
+      obtain ST' LT' where
+        phi': "phi C sig ! handler = Some (ST', LT')" and
+        less: "G \<turnstile> ([Class (Xcpt NullPointer)], LT) <=s (ST', LT')" and
+        pc':  "handler < length ins"
+        by (simp add: xcpt_eff_def) blast
+      note phi'
+      moreover
+      { from xcp
+        have "G,hp \<turnstile> xcp ::\<preceq> Class (Xcpt NullPointer)"
+          by (simp add: conf_def obj_ty_def system_xcpt_allocated)
+        moreover
+        from wf less loc
+        have "approx_loc G hp loc LT'"
+          by (simp add: sup_state_conv) blast        
+        moreover
+        note wf less pc' len 
+        ultimately
+        have "correct_frame G hp (ST',LT') maxl ins ?f'"
+          by (unfold correct_frame_def) (auto simp add: sup_state_conv 
+              approx_stk_def approx_val_def split: err.split elim: conf_widen)
+      }
+      ultimately
+      show ?thesis by (rule that)
+    next
+      case Putfield
+      with some_handler xp'
+      have xcp: "xcp = Addr (XcptRef NullPointer)"
+        by (simp add: raise_system_xcpt_def split_beta split: split_if_asm)
+      hence "cname_of hp xcp = Xcpt NullPointer" 
+        by (simp add: system_xcpt_allocated)
+      with Putfield some_handler phi_pc eff 
+      obtain ST' LT' where
+        phi': "phi C sig ! handler = Some (ST', LT')" and
+        less: "G \<turnstile> ([Class (Xcpt NullPointer)], LT) <=s (ST', LT')" and
+        pc':  "handler < length ins"
+        by (simp add: xcpt_eff_def) blast
+      note phi'
+      moreover
+      { from xcp
+        have "G,hp \<turnstile> xcp ::\<preceq> Class (Xcpt NullPointer)"
+          by (simp add: conf_def obj_ty_def system_xcpt_allocated)
+        moreover
+        from wf less loc
+        have "approx_loc G hp loc LT'"
+          by (simp add: sup_state_conv) blast        
+        moreover
+        note wf less pc' len 
+        ultimately
+        have "correct_frame G hp (ST',LT') maxl ins ?f'"
+          by (unfold correct_frame_def) (auto simp add: sup_state_conv 
+              approx_stk_def approx_val_def split: err.split elim: conf_widen)
+      }
+      ultimately
+      show ?thesis by (rule that)
+    next
+      case Checkcast
+      with some_handler xp'
+      have xcp: "xcp = Addr (XcptRef ClassCast)"
+        by (simp add: raise_system_xcpt_def split_beta split: split_if_asm)
+      hence "cname_of hp xcp = Xcpt ClassCast" 
+        by (simp add: system_xcpt_allocated)
+      with Checkcast some_handler phi_pc eff 
+      obtain ST' LT' where
+        phi': "phi C sig ! handler = Some (ST', LT')" and
+        less: "G \<turnstile> ([Class (Xcpt ClassCast)], LT) <=s (ST', LT')" and
+        pc':  "handler < length ins"
+        by (simp add: xcpt_eff_def) blast
+      note phi'
+      moreover
+      { from xcp
+        have "G,hp \<turnstile> xcp ::\<preceq> Class (Xcpt ClassCast)"
+          by (simp add: conf_def obj_ty_def system_xcpt_allocated)
+        moreover
+        from wf less loc
+        have "approx_loc G hp loc LT'"
+          by (simp add: sup_state_conv) blast        
+        moreover
+        note wf less pc' len 
+        ultimately
+        have "correct_frame G hp (ST',LT') maxl ins ?f'"
+          by (unfold correct_frame_def) (auto simp add: sup_state_conv 
+              approx_stk_def approx_val_def split: err.split elim: conf_widen)
+      }
+      ultimately
+      show ?thesis by (rule that)
+    next
+      case Invoke
+      with phi_pc eff 
+      have 
+        "\<forall>D\<in>set (match_any G pc et). 
+        the (?m D) < length ins \<and> G \<turnstile> Some ([Class D], LT) <=' phi C sig!the (?m D)"
+        by (simp add: xcpt_eff_def)
+      moreover
+      from some_handler
+      obtain D where
+        "D \<in> set (match_any G pc et)" and
+        D: "G \<turnstile> cname_of hp xcp \<preceq>C D" and
+        "?m D = Some handler"
+        by (blast dest: in_match_any)
+      ultimately
+      obtain 
+        pc': "handler < length ins" and
+        "G \<turnstile> Some ([Class D], LT) <=' phi C sig ! handler"
+        by auto
+      then
+      obtain ST' LT' where
+        phi': "phi C sig ! handler = Some (ST', LT')" and
+        less: "G \<turnstile> ([Class D], LT) <=s (ST', LT')" 
+        by auto
+      from xp wt correct
+      obtain addr T where
+        xcp: "xcp = Addr addr" "hp addr = Some T"
+        by (blast dest: exec_instr_xcpt_hp)
+      note phi'
+      moreover
+      { from xcp D
+        have "G,hp \<turnstile> xcp ::\<preceq> Class D"
+          by (simp add: conf_def obj_ty_def)
+        moreover
+        from wf less loc
+        have "approx_loc G hp loc LT'"
+          by (simp add: sup_state_conv) blast        
+        moreover
+        note wf less pc' len 
+        ultimately
+        have "correct_frame G hp (ST',LT') maxl ins ?f'"
+          by (unfold correct_frame_def) (auto simp add: sup_state_conv 
+              approx_stk_def approx_val_def split: err.split elim: conf_widen)
+      }
+      ultimately
+      show ?thesis by (rule that)
+    next
+      case Throw
+      with phi_pc eff 
+      have 
+        "\<forall>D\<in>set (match_any G pc et). 
+        the (?m D) < length ins \<and> G \<turnstile> Some ([Class D], LT) <=' phi C sig!the (?m D)"
+        by (simp add: xcpt_eff_def)
+      moreover
+      from some_handler
+      obtain D where
+        "D \<in> set (match_any G pc et)" and
+        D: "G \<turnstile> cname_of hp xcp \<preceq>C D" and
+        "?m D = Some handler"
+        by (blast dest: in_match_any)
+      ultimately
+      obtain 
+        pc': "handler < length ins" and
+        "G \<turnstile> Some ([Class D], LT) <=' phi C sig ! handler"
+        by auto
+      then
+      obtain ST' LT' where
+        phi': "phi C sig ! handler = Some (ST', LT')" and
+        less: "G \<turnstile> ([Class D], LT) <=s (ST', LT')" 
+        by auto
+      from xp wt correct
+      obtain addr T where
+        xcp: "xcp = Addr addr" "hp addr = Some T"
+        by (blast dest: exec_instr_xcpt_hp)
+      note phi'
+      moreover
+      { from xcp D
+        have "G,hp \<turnstile> xcp ::\<preceq> Class D"
+          by (simp add: conf_def obj_ty_def)
+        moreover
+        from wf less loc
+        have "approx_loc G hp loc LT'"
+          by (simp add: sup_state_conv) blast        
+        moreover
+        note wf less pc' len 
+        ultimately
+        have "correct_frame G hp (ST',LT') maxl ins ?f'"
+          by (unfold correct_frame_def) (auto simp add: sup_state_conv 
+              approx_stk_def approx_val_def split: err.split elim: conf_widen)
+      }
+      ultimately
+      show ?thesis by (rule that)
+    qed (insert xp', auto) -- "the other instructions don't generate exceptions"
+
+    from state' meth hp_ok class frames phi_pc' frame' 
+    have ?thesis by (unfold correct_state_def) simp
+  }
+  ultimately
+  show ?thesis by (cases "?match") blast+ 
+qed
+
+
+
 section {* Single Instructions *}
+
+text {*
+  In this section we look at each single (welltyped) instruction, and
+  prove that the state after execution of the instruction still conforms.
+  Since we have already handled exceptions above, we can now assume, that
+  on exception occurs for this (single step) execution.
+*}
 
 lemmas [iff] = not_Err_eq
 
 lemma Load_correct:
 "[| wf_prog wt G;
-    method (G,C) sig = Some (C,rT,maxs,maxl,ins); 
+    method (G,C) sig = Some (C,rT,maxs,maxl,ins,et); 
     ins!pc = Load idx; 
-    wt_instr (ins!pc) G rT (phi C sig) maxs (length ins) pc; 
+    wt_instr (ins!pc) G rT (phi C sig) maxs (length ins) et pc; 
     Some state' = exec (G, None, hp, (stk,loc,C,sig,pc)#frs); 
-    G,phi \<turnstile>JVM (None, hp, (stk,loc,C,sig,pc)#frs)\<surd> |] 
+    G,phi \<turnstile>JVM (None, hp, (stk,loc,C,sig,pc)#frs)\<surd> |]
 ==> G,phi \<turnstile>JVM state'\<surd>"
 apply (clarsimp simp add: defs1 map_eq_Cons)
 apply (blast intro: approx_loc_imp_approx_val_sup)
@@ -44,9 +596,9 @@ done
 
 lemma Store_correct:
 "[| wf_prog wt G;
-  method (G,C) sig = Some (C,rT,maxs,maxl,ins);
+  method (G,C) sig = Some (C,rT,maxs,maxl,ins,et);
   ins!pc = Store idx;
-  wt_instr (ins!pc) G rT (phi C sig) maxs (length ins) pc;
+  wt_instr (ins!pc) G rT (phi C sig) maxs (length ins) et pc;
   Some state' = exec (G, None, hp, (stk,loc,C,sig,pc)#frs);
   G,phi \<turnstile>JVM (None, hp, (stk,loc,C,sig,pc)#frs)\<surd> |]
 ==> G,phi \<turnstile>JVM state'\<surd>"
@@ -57,9 +609,9 @@ done
 
 lemma LitPush_correct:
 "[| wf_prog wt G;
-    method (G,C) sig = Some (C,rT,maxs,maxl,ins); 
+    method (G,C) sig = Some (C,rT,maxs,maxl,ins,et); 
     ins!pc = LitPush v;
-    wt_instr (ins!pc) G rT (phi C sig) maxs (length ins) pc; 
+    wt_instr (ins!pc) G rT (phi C sig) maxs (length ins) et pc; 
     Some state' = exec (G, None, hp, (stk,loc,C,sig,pc)#frs);
     G,phi \<turnstile>JVM (None, hp, (stk,loc,C,sig,pc)#frs)\<surd> |]
 ==> G,phi \<turnstile>JVM state'\<surd>" 
@@ -81,30 +633,33 @@ apply (cases v)
 apply (auto intro: rtrancl_trans)
 done
 
+lemmas defs1 = defs1 raise_system_xcpt_def
 
 lemma Checkcast_correct:
-"[| wf_prog wt G;
-    method (G,C) sig = Some (C,rT,maxs,maxl,ins); 
+"[| wt_jvm_prog G phi;
+    method (G,C) sig = Some (C,rT,maxs,maxl,ins,et); 
     ins!pc = Checkcast D; 
-    wt_instr (ins!pc) G rT (phi C sig) maxs (length ins) pc; 
+    wt_instr (ins!pc) G rT (phi C sig) maxs (length ins) et pc; 
     Some state' = exec (G, None, hp, (stk,loc,C,sig,pc)#frs) ; 
-    G,phi \<turnstile>JVM (None, hp, (stk,loc,C,sig,pc)#frs)\<surd> |] 
+    G,phi \<turnstile>JVM (None, hp, (stk,loc,C,sig,pc)#frs)\<surd>;
+    fst (exec_instr (ins!pc) G hp stk loc C sig pc frs) = None |] 
 ==> G,phi \<turnstile>JVM state'\<surd>"
-apply (clarsimp simp add: defs1 map_eq_Cons raise_xcpt_def)
+apply (clarsimp simp add: defs1 wt_jvm_prog_def map_eq_Cons split: split_if_asm)
 apply (blast intro: Cast_conf2)
 done
 
 
 lemma Getfield_correct:
-"[| wf_prog wt G;
-  method (G,C) sig = Some (C,rT,maxs,maxl,ins); 
+"[| wt_jvm_prog G phi;
+  method (G,C) sig = Some (C,rT,maxs,maxl,ins,et); 
   ins!pc = Getfield F D; 
-  wt_instr (ins!pc) G rT (phi C sig) maxs (length ins) pc; 
+  wt_instr (ins!pc) G rT (phi C sig) maxs (length ins) et pc; 
   Some state' = exec (G, None, hp, (stk,loc,C,sig,pc)#frs) ; 
-  G,phi \<turnstile>JVM (None, hp, (stk,loc,C,sig,pc)#frs)\<surd> |] 
+  G,phi \<turnstile>JVM (None, hp, (stk,loc,C,sig,pc)#frs)\<surd>;
+  fst (exec_instr (ins!pc) G hp stk loc C sig pc frs) = None |] 
 ==> G,phi \<turnstile>JVM state'\<surd>"
-apply (clarsimp simp add: defs1 raise_xcpt_def map_eq_Cons
-                split: option.split)
+apply (clarsimp simp add: defs1 map_eq_Cons wt_jvm_prog_def 
+                split: option.split split_if_asm)
 apply (frule conf_widen)
 apply assumption+
 apply (drule conf_RefTD)
@@ -112,19 +667,30 @@ apply (clarsimp simp add: defs1)
 apply (rule conjI)
  apply (drule widen_cfs_fields)
  apply assumption+
- apply (force intro: conf_widen simp add: hconf_def oconf_def lconf_def)
+ apply (erule conf_widen)
+ prefer 2
+  apply assumption
+ apply (simp add: hconf_def oconf_def lconf_def)
+ apply (elim allE)
+ apply (erule impE, assumption)
+ apply simp
+ apply (elim allE)
+ apply (erule impE, assumption)
+ apply clarsimp
 apply blast
 done
 
+
 lemma Putfield_correct:
 "[| wf_prog wt G;
-  method (G,C) sig = Some (C,rT,maxs,maxl,ins); 
+  method (G,C) sig = Some (C,rT,maxs,maxl,ins,et); 
   ins!pc = Putfield F D; 
-  wt_instr (ins!pc) G rT (phi C sig) maxs (length ins) pc; 
+  wt_instr (ins!pc) G rT (phi C sig) maxs (length ins) et pc; 
   Some state' = exec (G, None, hp, (stk,loc,C,sig,pc)#frs) ; 
-  G,phi \<turnstile>JVM (None, hp, (stk,loc,C,sig,pc)#frs)\<surd> |] 
+  G,phi \<turnstile>JVM (None, hp, (stk,loc,C,sig,pc)#frs)\<surd>;
+  fst (exec_instr (ins!pc) G hp stk loc C sig pc frs) = None |] 
 ==> G,phi \<turnstile>JVM state'\<surd>"
-apply (clarsimp simp add: defs1 raise_xcpt_def split: option.split List.split)
+apply (clarsimp simp add: defs1 split_beta split: option.split List.split split_if_asm)
 apply (frule conf_widen)
 prefer 2
   apply assumption
@@ -140,22 +706,25 @@ apply (blast
        dest: 
          widen_cfs_fields)
 done
+    
 
 lemma New_correct:
 "[| wf_prog wt G;
-  method (G,C) sig = Some (C,rT,maxs,maxl,ins); 
+  method (G,C) sig = Some (C,rT,maxs,maxl,ins,et); 
   ins!pc = New X; 
-  wt_instr (ins!pc) G rT (phi C sig) maxs (length ins) pc; 
+  wt_instr (ins!pc) G rT (phi C sig) maxs (length ins) et pc; 
   Some state' = exec (G, None, hp, (stk,loc,C,sig,pc)#frs) ; 
-  G,phi \<turnstile>JVM (None, hp, (stk,loc,C,sig,pc)#frs)\<surd> |] 
+  G,phi \<turnstile>JVM (None, hp, (stk,loc,C,sig,pc)#frs)\<surd>;
+  fst (exec_instr (ins!pc) G hp stk loc C sig pc frs) = None |] 
 ==> G,phi \<turnstile>JVM state'\<surd>"
 proof -
   assume wf:   "wf_prog wt G"
-  assume meth: "method (G,C) sig = Some (C,rT,maxs,maxl,ins)"
+  assume meth: "method (G,C) sig = Some (C,rT,maxs,maxl,ins,et)"
   assume ins:  "ins!pc = New X"
-  assume wt:   "wt_instr (ins!pc) G rT (phi C sig) maxs (length ins) pc"
+  assume wt:   "wt_instr (ins!pc) G rT (phi C sig) maxs (length ins) et pc"
   assume exec: "Some state' = exec (G, None, hp, (stk,loc,C,sig,pc)#frs)"
   assume conf: "G,phi \<turnstile>JVM (None, hp, (stk,loc,C,sig,pc)#frs)\<surd>"
+  assume no_x: "fst (exec_instr (ins!pc) G hp stk loc C sig pc frs) = None"
 
   from ins conf meth
   obtain ST LT where
@@ -169,75 +738,68 @@ proof -
   from phi_pc ins wt
   obtain ST' LT' where
     is_class_X: "is_class G X" and
+    maxs:       "length ST < maxs" and
     suc_pc:     "Suc pc < length ins" and
     phi_suc:    "phi C sig ! Suc pc = Some (ST', LT')" and
     less:       "G \<turnstile> (Class X # ST, LT) <=s (ST', LT')"
-    by (unfold wt_instr_def step_def) auto
+    by (unfold wt_instr_def eff_def norm_eff_def) auto
  
   obtain oref xp' where
-    new_Addr: "(oref,xp') = new_Addr hp"
-    by (cases "new_Addr hp") auto  
-  hence cases: 
-    "hp oref = None \<and> xp' = None \<or> xp' = Some OutOfMemory"
-    by (blast dest: new_AddrD)
+    new_Addr: "new_Addr hp = (oref,xp')"
+    by (cases "new_Addr hp") 
+  with ins no_x
+  obtain hp: "hp oref = None" and "xp' = None"
+    by (auto dest: new_AddrD simp add: raise_system_xcpt_def)
+  
+  with exec ins meth new_Addr 
+  have state':
+    "state' = Norm (hp(oref\<mapsto>(X, init_vars (fields (G, X)))), 
+              (Addr oref # stk, loc, C, sig, Suc pc) # frs)" 
+    (is "state' = Norm (?hp', ?f # frs)")
+    by simp    
   moreover
-  { assume "xp' = Some OutOfMemory"
-    with exec ins meth new_Addr [symmetric]
-    have "state' = (Some OutOfMemory, hp, (stk,loc,C,sig,Suc pc)#frs)" by simp
-    hence ?thesis by (simp add: correct_state_def)
-  }
+  from wf hp heap_ok is_class_X
+  have hp': "G \<turnstile>h ?hp' \<surd>"
+    by - (rule hconf_newref, auto simp add: oconf_def dest: fields_is_type)
   moreover
-  { assume hp: "hp oref = None" and "xp' = None"
-    with exec ins meth new_Addr [symmetric]
-    have state':
-      "state' = Norm (hp(oref\<mapsto>(X, init_vars (fields (G, X)))), 
-                      (Addr oref # stk, loc, C, sig, Suc pc) # frs)" 
-      (is "state' = Norm (?hp', ?f # frs)")
-      by simp    
-    moreover
-    from wf hp heap_ok is_class_X
-    have hp': "G \<turnstile>h ?hp' \<surd>"
-      by - (rule hconf_newref, 
-            auto simp add: oconf_def dest: fields_is_type)
-    moreover
-    from hp
-    have sup: "hp \<le>| ?hp'" by (rule hext_new)
-    from hp frame less suc_pc wf
-    have "correct_frame G ?hp' (ST', LT') maxl ins ?f"
-      apply (unfold correct_frame_def sup_state_conv)
-      apply (clarsimp simp add: map_eq_Cons conf_def fun_upd_apply approx_val_def)
-      apply (blast intro: approx_stk_sup_heap approx_loc_sup_heap sup)
-      done      
-    moreover
-    from hp frames wf heap_ok is_class_X
-    have "correct_frames G ?hp' phi rT sig frs"
-      by - (rule correct_frames_newref,
-            auto simp add: oconf_def dest: fields_is_type)
-    ultimately
-    have ?thesis
-      by (simp add: is_class_C meth phi_suc correct_state_def del: not_None_eq)
-  }
+  from hp
+  have sup: "hp \<le>| ?hp'" by (rule hext_new)
+  from hp frame less suc_pc wf
+  have "correct_frame G ?hp' (ST', LT') maxl ins ?f"
+    apply (unfold correct_frame_def sup_state_conv)
+    apply (clarsimp simp add: map_eq_Cons conf_def fun_upd_apply approx_val_def)
+    apply (blast intro: approx_stk_sup_heap approx_loc_sup_heap sup)
+    done      
+  moreover
+  from hp frames wf heap_ok is_class_X
+  have "correct_frames G ?hp' phi rT sig frs"
+    by - (rule correct_frames_newref, 
+          auto simp add: oconf_def dest: fields_is_type)
   ultimately
-  show ?thesis by auto
+  show ?thesis
+    by (simp add: is_class_C meth phi_suc correct_state_def del: not_None_eq)
 qed
 
 lemmas [simp del] = split_paired_Ex
 
+
 lemma Invoke_correct: 
 "[| wt_jvm_prog G phi; 
-  method (G,C) sig = Some (C,rT,maxs,maxl,ins); 
+  method (G,C) sig = Some (C,rT,maxs,maxl,ins,et); 
   ins ! pc = Invoke C' mn pTs; 
-  wt_instr (ins!pc) G rT (phi C sig) maxs (length ins) pc; 
+  wt_instr (ins!pc) G rT (phi C sig) maxs (length ins) et pc; 
   Some state' = exec (G, None, hp, (stk,loc,C,sig,pc)#frs) ; 
-  G,phi \<turnstile>JVM (None, hp, (stk,loc,C,sig,pc)#frs)\<surd> |] 
+  G,phi \<turnstile>JVM (None, hp, (stk,loc,C,sig,pc)#frs)\<surd>;
+  fst (exec_instr (ins!pc) G hp stk loc C sig pc frs) = None |] 
 ==> G,phi \<turnstile>JVM state'\<surd>" 
 proof -
   assume wtprog: "wt_jvm_prog G phi"
-  assume method: "method (G,C) sig = Some (C,rT,maxs,maxl,ins)"
+  assume method: "method (G,C) sig = Some (C,rT,maxs,maxl,ins,et)"
   assume ins:    "ins ! pc = Invoke C' mn pTs"
-  assume wti:    "wt_instr (ins!pc) G rT (phi C sig) maxs (length ins) pc"
+  assume wti:    "wt_instr (ins!pc) G rT (phi C sig) maxs (length ins) et pc"
   assume state': "Some state' = exec (G, None, hp, (stk,loc,C,sig,pc)#frs)"
   assume approx: "G,phi \<turnstile>JVM (None, hp, (stk,loc,C,sig,pc)#frs)\<surd>"
+  assume no_xcp: "fst (exec_instr (ins!pc) G hp stk loc C sig pc frs) = None"
   
   from wtprog 
   obtain wfmb where
@@ -262,18 +824,19 @@ proof -
     w:  "\<forall>x\<in>set (zip apTs pTs). x \<in> widen G" and
     mC':"method (G, C') (mn, pTs) = Some (D', rT, body)" and
     pc: "Suc pc < length ins" and
-    step: "G \<turnstile> step (Invoke C' mn pTs) G (Some s) <=' phi C sig!Suc pc"
-    by (simp add: wt_instr_def del: not_None_eq) (elim exE conjE, rule that)
+    eff: "G \<turnstile> norm_eff (Invoke C' mn pTs) G (Some s) <=' phi C sig!Suc pc"
+    by (simp add: wt_instr_def eff_def del: not_None_eq) 
+       (elim exE conjE, rule that)
 
-  from step
+  from eff
   obtain ST' LT' where
     s': "phi C sig ! Suc pc = Some (ST', LT')"
-    by (auto simp add: step_def split_paired_Ex)
+    by (simp add: norm_eff_def split_paired_Ex) blast
 
-  from X
+  from X 
   obtain T where
     X_Ref: "X = RefT T"
-    by (blast dest: widen_RefT2)
+    by - (drule widen_RefT2, erule exE, rule that)
   
   from s ins frame 
   obtain 
@@ -289,194 +852,245 @@ proof -
     a_stk': "approx_stk G hp stk' ST" and
     stk':   "stk = opTs @ oX # stk'" and
     l_o:    "length opTs = length apTs" 
-            "length stk' = length ST"
-    by (auto dest: approx_stk_append)
+            "length stk' = length ST"  
+    by - (drule approx_stk_append, auto)
 
-  from oX 
-  have "\<exists>T'. typeof (option_map obj_ty \<circ> hp) oX = Some T' \<and> G \<turnstile> T' \<preceq> X"
-    by (clarsimp simp add: approx_val_def conf_def)
-
-  with X_Ref
-  obtain T' where
-    oX_Ref: "typeof (option_map obj_ty \<circ> hp) oX = Some (RefT T')"
-            "G \<turnstile> RefT T' \<preceq> X"
-    by (auto dest: widen_RefT2)
+  from oX X_Ref
+  have oX_conf: "G,hp \<turnstile> oX ::\<preceq> RefT T"
+    by (simp add: approx_val_def)
 
   from stk' l_o l
   have oX_pos: "last (take (Suc (length pTs)) stk) = oX" by simp
 
-  with state' method ins 
-  have Null_ok: "oX = Null ==> ?thesis"
-    by (simp add: correct_state_def raise_xcpt_def)
+  with state' method ins no_xcp oX_conf
+  obtain ref where oX_Addr: "oX = Addr ref"
+    by (auto simp add: raise_system_xcpt_def dest: conf_RefTD)
+
+  with oX_conf X_Ref
+  obtain obj D where
+    loc:    "hp ref = Some obj" and
+    obj_ty: "obj_ty obj = Class D" and
+    D:      "G \<turnstile> Class D \<preceq> X"
+    by (auto simp add: conf_def) blast
   
-  { fix ref assume oX_Addr: "oX = Addr ref"
-    
-    with oX_Ref
-    obtain obj where
-      loc: "hp ref = Some obj" "obj_ty obj = RefT T'"
-      by auto
-
-    then 
-    obtain D where
-      obj_ty: "obj_ty obj = Class D"
-      by (auto simp add: obj_ty_def)
-
-    with X_Ref oX_Ref loc
-    obtain D: "G \<turnstile> Class D \<preceq> X"
-      by simp
-
-    with X_Ref
-    obtain X' where 
-      X': "X = Class X'"
-      by (blast dest: widen_Class)
+  with X_Ref obtain X' where X': "X = Class X'"
+    by (blast dest: widen_Class)
       
-    with X
-    have X'_subcls: "G \<turnstile> X' \<preceq>C C'" 
-      by simp
+  with X have X'_subcls: "G \<turnstile> X' \<preceq>C C'"  by simp
 
-    with mC' wfprog
-    obtain D0 rT0 maxs0 maxl0 ins0 where
-      mX: "method (G, X') (mn, pTs) = Some (D0, rT0, maxs0, maxl0, ins0)" "G\<turnstile>rT0\<preceq>rT"
-      by (fast dest: subtype_widen_methd)
-
-    from X' D
-    have D_subcls: "G \<turnstile> D \<preceq>C X'" 
-      by simp
-
-    with wfprog mX
-    obtain D'' rT' mxs' mxl' ins' where
-      mD: "method (G, D) (mn, pTs) = Some (D'', rT', mxs', mxl', ins')" 
-          "G \<turnstile> rT' \<preceq> rT0"
-      by (fast dest: subtype_widen_methd)
-
-    from mX mD
-    have rT': "G \<turnstile> rT' \<preceq> rT"
-      by - (rule widen_trans)
+  with mC' wfprog
+  obtain D0 rT0 maxs0 maxl0 ins0 et0 where
+    mX: "method (G, X') (mn, pTs) = Some (D0, rT0, maxs0, maxl0, ins0, et0)" "G\<turnstile>rT0\<preceq>rT"
+    by (auto dest: subtype_widen_methd intro: that)
     
-    from is_class X'_subcls D_subcls
-    have is_class_D: "is_class G D"
-      by (auto dest: subcls_is_class2)
-
-    with mD wfprog
-    obtain mD'': 
-      "method (G, D'') (mn, pTs) = Some (D'', rT', mxs', mxl', ins')"
-      "is_class G D''"
-      by (auto dest: method_in_md)
-      
-    from loc obj_ty
-    have "fst (the (hp ref)) = D"
-      by (simp add: obj_ty_def)
-
-    with oX_Addr oX_pos state' method ins stk' l_o l loc obj_ty mD 
-    have state'_val:
-      "state' =
-       Norm (hp, ([], Addr ref # rev opTs @ replicate mxl' arbitrary, 
-                  D'', (mn, pTs), 0) # (stk', loc, C, sig, Suc pc) # frs)"
-      (is "state' = Norm (hp, ?f # ?f' # frs)")
-      by (simp add: raise_xcpt_def)
-    
-    from wtprog mD''
-    have start: "wt_start G D'' pTs mxl' (phi D'' (mn, pTs)) \<and> ins' \<noteq> []"
-      by (auto dest: wt_jvm_prog_impl_wt_start)
-    
-    then
-    obtain LT0 where
-      LT0: "phi D'' (mn, pTs) ! 0 = Some ([], LT0)"
-      by (clarsimp simp add: wt_start_def sup_state_conv)
-
-    have c_f: "correct_frame G hp ([], LT0) mxl' ins' ?f"
-    proof -
-      from start LT0
-      have sup_loc: 
-        "G \<turnstile> (OK (Class D'') # map OK pTs @ replicate mxl' Err) <=l LT0"
-        (is "G \<turnstile> ?LT <=l LT0")
-        by (simp add: wt_start_def sup_state_conv)
-
-      have r: "approx_loc G hp (replicate mxl' arbitrary) (replicate mxl' Err)"
-        by (simp add: approx_loc_def approx_val_Err 
-                      list_all2_def set_replicate_conv_if)
-
-      from wfprog mD is_class_D
-      have "G \<turnstile> Class D \<preceq> Class D''"
-        by (auto dest: method_wf_mdecl)
-      with obj_ty loc
-      have a: "approx_val G hp (Addr ref) (OK (Class D''))"
-        by (simp add: approx_val_def conf_def)
-
-      from opTs w l l_o wfprog 
-      have "approx_stk G hp opTs (rev pTs)" 
-	by (auto elim!: approx_stk_all_widen simp add: zip_rev)
-      hence "approx_stk G hp (rev opTs) pTs" by (subst approx_stk_rev)
-
-      with r a l_o l
-      have "approx_loc G hp (Addr ref # rev opTs @ replicate mxl' arbitrary) ?LT"
-        (is "approx_loc G hp ?lt ?LT")
-        by (auto simp add: approx_loc_append approx_stk_def)
-
-      from this sup_loc wfprog
-      have "approx_loc G hp ?lt LT0" by (rule approx_loc_widen)
-      with start l_o l
-      show ?thesis by (simp add: correct_frame_def)
-    qed
-
-    have c_f': "correct_frame G hp (tl ST', LT') maxl ins ?f'"
-    proof -    
-      from s s' mC' step l
-      have "G \<turnstile> LT <=l LT'"
-        by (simp add: step_def sup_state_conv)
-      with wfprog a_loc
-      have a: "approx_loc G hp loc LT'"
-        by - (rule approx_loc_widen)
-      moreover
-      from s s' mC' step l
-      have  "G \<turnstile> map OK ST <=l map OK (tl ST')"
-        by (auto simp add: step_def sup_state_conv map_eq_Cons)
-      with wfprog a_stk'
-      have "approx_stk G hp stk' (tl ST')"
-        by - (rule approx_stk_widen)
-      ultimately
-      show ?thesis by (simp add: correct_frame_def suc_l pc)
-    qed
-
-    with state'_val heap_ok mD'' ins method phi_pc s X' l 
-         frames s' LT0 c_f c_f' is_class_C
-    have ?thesis by (simp add: correct_state_def) (intro exI conjI, blast)
-  }
+  from X' D have D_subcls: "G \<turnstile> D \<preceq>C X'" by simp
   
-  with Null_ok oX_Ref
-  show "G,phi \<turnstile>JVM state'\<surd>" by (cases oX) auto
+  with wfprog mX
+  obtain D'' rT' mxs' mxl' ins' et' where
+    mD: "method (G, D) (mn, pTs) = Some (D'', rT', mxs', mxl', ins', et')" 
+        "G \<turnstile> rT' \<preceq> rT0"
+    by (auto dest: subtype_widen_methd intro: that)
+  
+  from mX mD have rT': "G \<turnstile> rT' \<preceq> rT" by - (rule widen_trans)
+  
+  from is_class X'_subcls D_subcls
+  have is_class_D: "is_class G D" by (auto dest: subcls_is_class2)
+  
+  with mD wfprog
+  obtain mD'': 
+    "method (G, D'') (mn, pTs) = Some (D'', rT', mxs', mxl', ins', et')"
+    "is_class G D''"
+    by (auto dest: method_in_md)
+      
+  from loc obj_ty have "fst (the (hp ref)) = D" by (simp add: obj_ty_def)
+
+  with oX_Addr oX_pos state' method ins stk' l_o l loc obj_ty mD no_xcp
+  have state'_val:
+    "state' =
+     Norm (hp, ([], Addr ref # rev opTs @ replicate mxl' arbitrary, 
+                D'', (mn, pTs), 0) # (opTs @ Addr ref # stk', loc, C, sig, pc) # frs)"
+    (is "state' = Norm (hp, ?f # ?f' # frs)")
+    by (simp add: raise_system_xcpt_def)
+    
+  from wtprog mD''
+  have start: "wt_start G D'' pTs mxl' (phi D'' (mn, pTs)) \<and> ins' \<noteq> []"
+    by (auto dest: wt_jvm_prog_impl_wt_start)
+    
+  then obtain LT0 where
+    LT0: "phi D'' (mn, pTs) ! 0 = Some ([], LT0)"
+    by (clarsimp simp add: wt_start_def sup_state_conv)
+
+  have c_f: "correct_frame G hp ([], LT0) mxl' ins' ?f"
+  proof -
+    from start LT0
+    have sup_loc: 
+      "G \<turnstile> (OK (Class D'') # map OK pTs @ replicate mxl' Err) <=l LT0"
+      (is "G \<turnstile> ?LT <=l LT0")
+      by (simp add: wt_start_def sup_state_conv)
+
+    have r: "approx_loc G hp (replicate mxl' arbitrary) (replicate mxl' Err)"
+      by (simp add: approx_loc_def list_all2_def set_replicate_conv_if)
+    
+    from wfprog mD is_class_D
+    have "G \<turnstile> Class D \<preceq> Class D''"
+      by (auto dest: method_wf_mdecl)
+    with obj_ty loc
+    have a: "approx_val G hp (Addr ref) (OK (Class D''))"
+      by (simp add: approx_val_def conf_def)
+
+    from opTs w l l_o wfprog 
+    have "approx_stk G hp opTs (rev pTs)" 
+      by (auto elim!: approx_stk_all_widen simp add: zip_rev)
+    hence "approx_stk G hp (rev opTs) pTs" by (subst approx_stk_rev)
+
+    with r a l_o l
+    have "approx_loc G hp (Addr ref # rev opTs @ replicate mxl' arbitrary) ?LT"
+      (is "approx_loc G hp ?lt ?LT")
+      by (auto simp add: approx_loc_append approx_stk_def)
+
+    from this sup_loc wfprog
+    have "approx_loc G hp ?lt LT0" by (rule approx_loc_widen)
+    with start l_o l
+    show ?thesis by (simp add: correct_frame_def)
+  qed
+
+  from state'_val heap_ok mD'' ins method phi_pc s X' l mX
+       frames s' LT0 c_f is_class_C stk' oX_Addr frame 
+  show ?thesis by (simp add: correct_state_def) (intro exI conjI, blast)
 qed
 
 lemmas [simp del] = map_append
 
 lemma Return_correct:
 "[| wt_jvm_prog G phi; 
-  method (G,C) sig = Some (C,rT,maxs,maxl,ins); 
+  method (G,C) sig = Some (C,rT,maxs,maxl,ins,et); 
   ins ! pc = Return; 
-  wt_instr (ins!pc) G rT (phi C sig) maxs (length ins) pc; 
+  wt_instr (ins!pc) G rT (phi C sig) maxs (length ins) et pc; 
   Some state' = exec (G, None, hp, (stk,loc,C,sig,pc)#frs) ; 
-  G,phi \<turnstile>JVM (None, hp, (stk,loc,C,sig,pc)#frs)\<surd> |] 
+  G,phi \<turnstile>JVM (None, hp, (stk,loc,C,sig,pc)#frs)\<surd> |]
 ==> G,phi \<turnstile>JVM state'\<surd>"
-apply (clarsimp simp add: neq_Nil_conv defs1 split: split_if_asm iff del: not_None_eq)
-apply (frule wt_jvm_prog_impl_wt_instr)
-apply (assumption, assumption, erule Suc_lessD)
-apply (clarsimp simp add: map_eq_Cons append_eq_conv_conj defs1)
-apply (unfold wt_jvm_prog_def)
-apply (frule subcls_widen_methd, assumption+)
-apply clarify
-apply simp
-apply (erule conf_widen, assumption)
-apply (erule widen_trans)+
-apply blast
-done
+proof -
+  assume wt_prog: "wt_jvm_prog G phi"
+  assume meth: "method (G,C) sig = Some (C,rT,maxs,maxl,ins,et)"
+  assume ins: "ins ! pc = Return"
+  assume wt: "wt_instr (ins!pc) G rT (phi C sig) maxs (length ins) et pc"
+  assume s': "Some state' = exec (G, None, hp, (stk,loc,C,sig,pc)#frs)"
+  assume correct: "G,phi \<turnstile>JVM (None, hp, (stk,loc,C,sig,pc)#frs)\<surd>"
 
+  from wt_prog 
+  obtain wfmb where wf: "wf_prog wfmb G" by (simp add: wt_jvm_prog_def)
+
+  from meth ins s'
+  have "frs = [] \<Longrightarrow> ?thesis" by (simp add: correct_state_def)
+  moreover
+  { fix f frs' 
+    assume frs': "frs = f#frs'"
+    moreover
+    obtain stk' loc' C' sig' pc' where
+      f: "f = (stk',loc',C',sig',pc')" by (cases f)
+    moreover
+    obtain mn pt where
+      sig: "sig = (mn,pt)" by (cases sig)
+    moreover
+    note meth ins s'
+    ultimately
+    have state':
+      "state' = (None,hp,(hd stk#(drop (1+length pt) stk'),loc',C',sig',pc'+1)#frs')"
+      (is "state' = (None,hp,?f'#frs')")
+      by simp
+    
+    from correct meth
+    obtain ST LT where
+      hp_ok:  "G \<turnstile>h hp \<surd>" and
+      phi_pc: "phi C sig ! pc = Some (ST, LT)" and
+      frame:  "correct_frame G hp (ST, LT) maxl ins (stk,loc,C,sig,pc)" and
+      frames: "correct_frames G hp phi rT sig frs"
+      by (simp add: correct_state_def, clarify, blast)    
+
+    from phi_pc ins wt
+    obtain T ST' where "ST = T # ST'" "G \<turnstile> T \<preceq> rT"
+      by (simp add: wt_instr_def) blast    
+    with wf frame 
+    have hd_stk: "G,hp \<turnstile> (hd stk) ::\<preceq> rT"
+      by (auto simp add: correct_frame_def elim: conf_widen)
+
+    from f frs' frames sig
+    obtain apTs ST0' ST' LT' D D' D'' rT' rT'' maxs' maxl' ins' et' body where
+      phi':   "phi C' sig' ! pc' = Some (ST',LT')" and
+      class': "is_class G C'" and
+      meth':  "method (G,C') sig' = Some (C',rT',maxs',maxl',ins',et')" and
+      ins':   "ins' ! pc' = Invoke D' mn pt" and
+      frame': "correct_frame G hp (ST', LT') maxl' ins' f" and
+      frames':"correct_frames G hp phi rT' sig' frs'" and
+      rT'':   "G \<turnstile> rT \<preceq> rT''" and
+      meth'': "method (G, D) sig = Some (D'', rT'', body)" and
+      ST0':   "ST' = rev apTs @ Class D # ST0'" and
+      len':   "length apTs = length pt" 
+      by clarsimp blast    
+
+    from f frame'
+    obtain
+      stk': "approx_stk G hp stk' ST'" and
+      loc': "approx_loc G hp loc' LT'" and
+      pc':  "pc' < length ins'" and
+      lloc':"length loc' = Suc (length (snd sig') + maxl')"
+      by (simp add: correct_frame_def)
+
+    from wt_prog class' meth' pc'  
+    have "wt_instr (ins'!pc') G rT' (phi C' sig') maxs' (length ins') et' pc'"
+      by (rule wt_jvm_prog_impl_wt_instr)
+    with ins' phi' sig
+    obtain apTs ST0 X ST'' LT'' body' rT0 mD where
+      phi_suc: "phi C' sig' ! Suc pc' = Some (ST'', LT'')" and
+      ST0:     "ST' = rev apTs @ X # ST0" and
+      len:     "length apTs = length pt" and
+      less:    "G \<turnstile> (rT0 # ST0, LT') <=s (ST'', LT'')" and
+      methD':  "method (G, D') sig = Some (mD, rT0, body')" and
+      lessD':  "G \<turnstile> X \<preceq> Class D'" and
+      suc_pc': "Suc pc' < length ins'"
+      by (clarsimp simp add: wt_instr_def eff_def norm_eff_def) blast
+
+    from len len' ST0 ST0'
+    have "X = Class D" by simp
+    with lessD'
+    have "G \<turnstile> D \<preceq>C D'" by simp
+    moreover
+    note wf meth'' methD'
+    ultimately
+    have "G \<turnstile> rT'' \<preceq> rT0" by (auto dest: subcls_widen_methd)
+    with wf hd_stk rT''
+    have hd_stk': "G,hp \<turnstile> (hd stk) ::\<preceq> rT0" by (auto elim: conf_widen widen_trans)
+        
+    have frame'':
+      "correct_frame G hp (ST'',LT'') maxl' ins' ?f'"
+    proof -
+      from wf hd_stk' len stk' less ST0
+      have "approx_stk G hp (hd stk # drop (1+length pt) stk') ST''" 
+        by (auto simp add: map_eq_Cons sup_state_conv
+                 dest!: approx_stk_append elim: conf_widen)
+      moreover
+      from wf loc' less
+      have "approx_loc G hp loc' LT''" by (simp add: sup_state_conv) blast
+      moreover
+      note suc_pc' lloc'
+      ultimately
+      show ?thesis by (simp add: correct_frame_def)
+    qed
+
+    with state' frs' f meth hp_ok hd_stk phi_suc frames' meth' phi' class'
+    have ?thesis by (simp add: correct_state_def)
+  }
+  ultimately
+  show ?thesis by (cases frs) blast+
+qed
+  
 lemmas [simp] = map_append
 
 lemma Goto_correct:
 "[| wf_prog wt G; 
-  method (G,C) sig = Some (C,rT,maxs,maxl,ins); 
+  method (G,C) sig = Some (C,rT,maxs,maxl,ins,et); 
   ins ! pc = Goto branch; 
-  wt_instr (ins!pc) G rT (phi C sig) maxs (length ins) pc; 
+  wt_instr (ins!pc) G rT (phi C sig) maxs (length ins) et pc; 
   Some state' = exec (G, None, hp, (stk,loc,C,sig,pc)#frs) ; 
   G,phi \<turnstile>JVM (None, hp, (stk,loc,C,sig,pc)#frs)\<surd> |] 
 ==> G,phi \<turnstile>JVM state'\<surd>"
@@ -487,9 +1101,9 @@ done
 
 lemma Ifcmpeq_correct:
 "[| wf_prog wt G; 
-  method (G,C) sig = Some (C,rT,maxs,maxl,ins); 
+  method (G,C) sig = Some (C,rT,maxs,maxl,ins,et); 
   ins ! pc = Ifcmpeq branch; 
-  wt_instr (ins!pc) G rT (phi C sig) maxs (length ins) pc; 
+  wt_instr (ins!pc) G rT (phi C sig) maxs (length ins) et pc; 
   Some state' = exec (G, None, hp, (stk,loc,C,sig,pc)#frs) ; 
   G,phi \<turnstile>JVM (None, hp, (stk,loc,C,sig,pc)#frs)\<surd> |] 
 ==> G,phi \<turnstile>JVM state'\<surd>"
@@ -499,9 +1113,9 @@ done
 
 lemma Pop_correct:
 "[| wf_prog wt G; 
-  method (G,C) sig = Some (C,rT,maxs,maxl,ins); 
+  method (G,C) sig = Some (C,rT,maxs,maxl,ins,et); 
   ins ! pc = Pop;
-  wt_instr (ins!pc) G rT (phi C sig) maxs (length ins) pc; 
+  wt_instr (ins!pc) G rT (phi C sig) maxs (length ins) et pc; 
   Some state' = exec (G, None, hp, (stk,loc,C,sig,pc)#frs) ; 
   G,phi \<turnstile>JVM (None, hp, (stk,loc,C,sig,pc)#frs)\<surd> |] 
 ==> G,phi \<turnstile>JVM state'\<surd>"
@@ -511,9 +1125,9 @@ done
 
 lemma Dup_correct:
 "[| wf_prog wt G; 
-  method (G,C) sig = Some (C,rT,maxs,maxl,ins); 
+  method (G,C) sig = Some (C,rT,maxs,maxl,ins,et); 
   ins ! pc = Dup;
-  wt_instr (ins!pc) G rT (phi C sig) maxs (length ins) pc; 
+  wt_instr (ins!pc) G rT (phi C sig) maxs (length ins) et pc; 
   Some state' = exec (G, None, hp, (stk,loc,C,sig,pc)#frs) ; 
   G,phi \<turnstile>JVM (None, hp, (stk,loc,C,sig,pc)#frs)\<surd> |] 
 ==> G,phi \<turnstile>JVM state'\<surd>"
@@ -523,9 +1137,9 @@ done
 
 lemma Dup_x1_correct:
 "[| wf_prog wt G; 
-  method (G,C) sig = Some (C,rT,maxs,maxl,ins); 
+  method (G,C) sig = Some (C,rT,maxs,maxl,ins,et); 
   ins ! pc = Dup_x1;
-  wt_instr (ins!pc) G rT (phi C sig) maxs (length ins) pc; 
+  wt_instr (ins!pc) G rT (phi C sig) maxs (length ins) et pc; 
   Some state' = exec (G, None, hp, (stk,loc,C,sig,pc)#frs) ; 
   G,phi \<turnstile>JVM (None, hp, (stk,loc,C,sig,pc)#frs)\<surd> |] 
 ==> G,phi \<turnstile>JVM state'\<surd>"
@@ -535,9 +1149,9 @@ done
 
 lemma Dup_x2_correct:
 "[| wf_prog wt G; 
-  method (G,C) sig = Some (C,rT,maxs,maxl,ins); 
+  method (G,C) sig = Some (C,rT,maxs,maxl,ins,et); 
   ins ! pc = Dup_x2;
-  wt_instr (ins!pc) G rT (phi C sig) maxs (length ins) pc; 
+  wt_instr (ins!pc) G rT (phi C sig) maxs (length ins) et pc; 
   Some state' = exec (G, None, hp, (stk,loc,C,sig,pc)#frs) ; 
   G,phi \<turnstile>JVM (None, hp, (stk,loc,C,sig,pc)#frs)\<surd> |] 
 ==> G,phi \<turnstile>JVM state'\<surd>"
@@ -547,9 +1161,9 @@ done
 
 lemma Swap_correct:
 "[| wf_prog wt G; 
-  method (G,C) sig = Some (C,rT,maxs,maxl,ins); 
+  method (G,C) sig = Some (C,rT,maxs,maxl,ins,et); 
   ins ! pc = Swap;
-  wt_instr (ins!pc) G rT (phi C sig) maxs (length ins) pc; 
+  wt_instr (ins!pc) G rT (phi C sig) maxs (length ins) et pc; 
   Some state' = exec (G, None, hp, (stk,loc,C,sig,pc)#frs) ; 
   G,phi \<turnstile>JVM (None, hp, (stk,loc,C,sig,pc)#frs)\<surd> |] 
 ==> G,phi \<turnstile>JVM state'\<surd>"
@@ -559,9 +1173,9 @@ done
 
 lemma IAdd_correct:
 "[| wf_prog wt G; 
-  method (G,C) sig = Some (C,rT,maxs,maxl,ins); 
+  method (G,C) sig = Some (C,rT,maxs,maxl,ins,et); 
   ins ! pc = IAdd; 
-  wt_instr (ins!pc) G rT (phi C sig) maxs (length ins) pc; 
+  wt_instr (ins!pc) G rT (phi C sig) maxs (length ins) et pc; 
   Some state' = exec (G, None, hp, (stk,loc,C,sig,pc)#frs) ; 
   G,phi \<turnstile>JVM (None, hp, (stk,loc,C,sig,pc)#frs)\<surd> |] 
 ==> G,phi \<turnstile>JVM state'\<surd>"
@@ -569,29 +1183,51 @@ apply (clarsimp simp add: defs1 map_eq_Cons approx_val_def conf_def)
 apply blast
 done
 
+lemma Throw_correct:
+"[| wf_prog wt G; 
+  method (G,C) sig = Some (C,rT,maxs,maxl,ins,et); 
+  ins ! pc = Throw; 
+  Some state' = exec (G, None, hp, (stk,loc,C,sig,pc)#frs) ; 
+  G,phi \<turnstile>JVM (None, hp, (stk,loc,C,sig,pc)#frs)\<surd>;
+  fst (exec_instr (ins!pc) G hp stk loc C sig pc frs) = None |] 
+==> G,phi \<turnstile>JVM state'\<surd>"
+  by simp
 
-lemma instr_correct:
+
+text {*
+  The next theorem collects the results of the sections above,
+  i.e.~exception handling and the execution step for each 
+  instruction. It states type safety for single step execution:
+  in welltyped programs, a conforming state is transformed
+  into another conforming state when one instruction is executed.
+*}
+theorem instr_correct:
 "[| wt_jvm_prog G phi;
-  method (G,C) sig = Some (C,rT,maxs,maxl,ins); 
+  method (G,C) sig = Some (C,rT,maxs,maxl,ins,et);
   Some state' = exec (G, None, hp, (stk,loc,C,sig,pc)#frs); 
   G,phi \<turnstile>JVM (None, hp, (stk,loc,C,sig,pc)#frs)\<surd> |] 
 ==> G,phi \<turnstile>JVM state'\<surd>"
 apply (frule wt_jvm_prog_impl_wt_instr_cor)
 apply assumption+
+apply (cases "fst (exec_instr (ins!pc) G hp stk loc C sig pc frs)")
+defer
+apply (erule xcpt_correct, assumption+) 
 apply (cases "ins!pc")
 prefer 8
 apply (rule Invoke_correct, assumption+)
 prefer 8
 apply (rule Return_correct, assumption+)
+prefer 5
+apply (rule Getfield_correct, assumption+)
+prefer 6
+apply (rule Checkcast_correct, assumption+)
 
 apply (unfold wt_jvm_prog_def)
 apply (rule Load_correct, assumption+)
 apply (rule Store_correct, assumption+)
 apply (rule LitPush_correct, assumption+)
 apply (rule New_correct, assumption+)
-apply (rule Getfield_correct, assumption+)
 apply (rule Putfield_correct, assumption+)
-apply (rule Checkcast_correct, assumption+)
 apply (rule Pop_correct, assumption+)
 apply (rule Dup_correct, assumption+)
 apply (rule Dup_x1_correct, assumption+)
@@ -600,6 +1236,7 @@ apply (rule Swap_correct, assumption+)
 apply (rule IAdd_correct, assumption+)
 apply (rule Goto_correct, assumption+)
 apply (rule Ifcmpeq_correct, assumption+)
+apply (rule Throw_correct, assumption+)
 done
 
 section {* Main *}
@@ -627,9 +1264,10 @@ apply simp_all
 done
 
 
+
 lemma L0:
   "[| xp=None; frs\<noteq>[] |] ==> (\<exists>state'. exec (G,xp,hp,frs) = Some state')"
-by (clarsimp simp add: neq_Nil_conv simp del: split_paired_Ex)
+by (clarsimp simp add: neq_Nil_conv split_beta)
 
 lemma L1:
   "[|wt_jvm_prog G phi; G,phi \<turnstile>JVM (xp,hp,frs)\<surd>; xp=None; frs\<noteq>[]|] 
@@ -639,7 +1277,6 @@ apply assumption
 apply (fast intro: BV_correct_1)
 done
 
-
 theorem BV_correct [rule_format]:
 "[| wt_jvm_prog G phi; G \<turnstile> s -jvm-> t |] ==> G,phi \<turnstile>JVM s\<surd> --> G,phi \<turnstile>JVM t\<surd>"
 apply (unfold exec_all_def)
@@ -648,12 +1285,11 @@ apply (erule rtrancl_induct)
 apply (auto intro: BV_correct_1)
 done
 
-
 theorem BV_correct_initial:
 "[| wt_jvm_prog G phi; 
     G \<turnstile> s0 -jvm-> (None,hp,(stk,loc,C,sig,pc)#frs); G,phi \<turnstile>JVM s0 \<surd>|] 
-==> approx_stk G hp stk (fst (the (((phi  C)  sig) ! pc))) \<and> 
-    approx_loc G hp loc (snd (the (((phi  C)  sig) ! pc)))"
+==> approx_stk G hp stk (fst (the (phi C sig ! pc))) \<and> 
+    approx_loc G hp loc (snd (the (phi C sig ! pc)))"
 apply (drule BV_correct)
 apply assumption+
 apply (simp add: correct_state_def correct_frame_def split_def 
