src/HOL/MicroJava/BV/Effect.thy
@@ -1,0 +1,339 @@
+(*  Title:      HOL/MicroJava/BV/Effect.thy
+    ID:         $Id$
+    Author:     Gerwin Klein
+    Copyright   2000 Technische Universitaet Muenchen
+*)
+
+header {* Effect of Instructions on the State Type *}
+
+theory Effect = JVMType + JVMExec:
+
+types
+  succ_type = "(p_count \<times> state_type option) list"
+
+text {* Program counter of successor instructions: *}
+consts
+  succs :: "instr => p_count => p_count list"
+primrec 
+  "succs (Load idx) pc         = [pc+1]"
+  "succs (Store idx) pc        = [pc+1]"
+  "succs (LitPush v) pc        = [pc+1]"
+  "succs (Getfield F C) pc     = [pc+1]"
+  "succs (Putfield F C) pc     = [pc+1]"
+  "succs (New C) pc            = [pc+1]"
+  "succs (Checkcast C) pc      = [pc+1]"
+  "succs Pop pc                = [pc+1]"
+  "succs Dup pc                = [pc+1]"
+  "succs Dup_x1 pc             = [pc+1]"
+  "succs Dup_x2 pc             = [pc+1]"
+  "succs Swap pc               = [pc+1]"
+  "succs IAdd pc               = [pc+1]"
+  "succs (Ifcmpeq b) pc        = [pc+1, nat (int pc + b)]"
+  "succs (Goto b) pc           = [nat (int pc + b)]"
+  "succs Return pc             = [pc]"  
+  "succs (Invoke C mn fpTs) pc = [pc+1]"
+  "succs Throw pc              = [pc]"
+
+text "Effect of instruction on the state type:"
+consts 
+eff' :: "instr \<times> jvm_prog \<times> state_type => state_type"
+
+recdef eff' "{}"
+"eff' (Load idx,  G, (ST, LT))          = (ok_val (LT ! idx) # ST, LT)"
+"eff' (Store idx, G, (ts#ST, LT))       = (ST, LT[idx:= OK ts])"
+"eff' (LitPush v, G, (ST, LT))           = (the (typeof (\<lambda>v. None) v) # ST, LT)"
+"eff' (Getfield F C, G, (oT#ST, LT))    = (snd (the (field (G,C) F)) # ST, LT)"
+"eff' (Putfield F C, G, (vT#oT#ST, LT)) = (ST,LT)"
+"eff' (New C, G, (ST,LT))               = (Class C # ST, LT)"
+"eff' (Checkcast C, G, (RefT rt#ST,LT)) = (Class C # ST,LT)"
+"eff' (Pop, G, (ts#ST,LT))              = (ST,LT)"
+"eff' (Dup, G, (ts#ST,LT))              = (ts#ts#ST,LT)"
+"eff' (Dup_x1, G, (ts1#ts2#ST,LT))      = (ts1#ts2#ts1#ST,LT)"
+"eff' (Dup_x2, G, (ts1#ts2#ts3#ST,LT))  = (ts1#ts2#ts3#ts1#ST,LT)"
+"eff' (Swap, G, (ts1#ts2#ST,LT))        = (ts2#ts1#ST,LT)"
+"eff' (IAdd, G, (PrimT Integer#PrimT Integer#ST,LT)) 
+                                         = (PrimT Integer#ST,LT)"
+"eff' (Ifcmpeq b, G, (ts1#ts2#ST,LT))   = (ST,LT)"
+"eff' (Goto b, G, s)                    = s"
+  -- "Return has no successor instruction in the same method"
+"eff' (Return, G, s)                    = s" 
+  -- "Throw always terminates abruptly"
+"eff' (Throw, G, s)                     = s"
+"eff' (Invoke C mn fpTs, G, (ST,LT))    = (let ST' = drop (length fpTs) ST 
+  in  (fst (snd (the (method (G,C) (mn,fpTs))))#(tl ST'),LT))" 
+
+
+consts
+  match_any :: "jvm_prog \<Rightarrow> p_count \<Rightarrow> exception_table \<Rightarrow> cname list"
+primrec
+  "match_any G pc [] = []"
+  "match_any G pc (e#es) = (let (start_pc, end_pc, handler_pc, catch_type) = e;
+                                es' = match_any G pc es 
+                            in 
+                            if start_pc <= pc \<and> pc < end_pc then catch_type#es' else es')"
+
+
+consts
+  xcpt_names :: "instr \<times> jvm_prog \<times> p_count \<times> exception_table => cname list" 
+recdef xcpt_names "{}"
+  "xcpt_names (Getfield F C, G, pc, et) = [Xcpt NullPointer]" 
+  "xcpt_names (Putfield F C, G, pc, et) = [Xcpt NullPointer]"
+  "xcpt_names (New C, G, pc, et)        = [Xcpt OutOfMemory]"
+  "xcpt_names (Checkcast C, G, pc, et)  = [Xcpt ClassCast]"
+  "xcpt_names (Throw, G, pc, et)        = match_any G pc et"
+  "xcpt_names (Invoke C m p, G, pc, et) = match_any G pc et" 
+  "xcpt_names (i, G, pc, et)            = []" 
+
+
+constdefs
+  xcpt_eff :: "instr \<Rightarrow> jvm_prog \<Rightarrow> p_count \<Rightarrow> state_type option \<Rightarrow> exception_table \<Rightarrow> succ_type"
+  "xcpt_eff i G pc s et == 
+   map (\<lambda>C. (the (match_exception_table G C pc et), case s of None \<Rightarrow> None | Some s' \<Rightarrow> Some ([Class C], snd s'))) 
+       (xcpt_names (i,G,pc,et))"
+
+  norm_eff :: "instr \<Rightarrow> jvm_prog \<Rightarrow> state_type option \<Rightarrow> state_type option"
+  "norm_eff i G == option_map (\<lambda>s. eff' (i,G,s))"
+
+  eff :: "instr => jvm_prog => p_count => exception_table => state_type option => succ_type"
+  "eff i G pc et s == (map (\<lambda>pc'. (pc',norm_eff i G s)) (succs i pc)) @ (xcpt_eff i G pc s et)"
+
+
+text "Conditions under which eff is applicable:"
+consts
+app' :: "instr \<times> jvm_prog \<times> nat \<times> ty \<times> state_type => bool"
+
+recdef app' "{}"
+"app' (Load idx, G, maxs, rT, s)                  = (idx < length (snd s) \<and> 
+                                                    (snd s) ! idx \<noteq> Err \<and> 
+                                                    length (fst s) < maxs)"
+"app' (Store idx, G, maxs, rT, (ts#ST, LT))       = (idx < length LT)"
+"app' (LitPush v, G, maxs, rT, s)                  = (length (fst s) < maxs \<and> typeof (\<lambda>t. None) v \<noteq> None)"
+"app' (Getfield F C, G, maxs, rT, (oT#ST, LT))    = (is_class G C \<and>
+                                              field (G,C) F \<noteq> None \<and>
+                                              fst (the (field (G,C) F)) = C \<and>
+                                              G \<turnstile> oT \<preceq> (Class C))"
+"app' (Putfield F C, G, maxs, rT, (vT#oT#ST, LT)) = (is_class G C \<and> 
+                                              field (G,C) F \<noteq> None \<and>
+                                              fst (the (field (G,C) F)) = C \<and>
+                                              G \<turnstile> oT \<preceq> (Class C) \<and>
+                                              G \<turnstile> vT \<preceq> (snd (the (field (G,C) F))))" 
+"app' (New C, G, maxs, rT, s)                     = (is_class G C \<and> length (fst s) < maxs)"
+"app' (Checkcast C, G, maxs, rT, (RefT rt#ST,LT)) = (is_class G C)"
+"app' (Pop, G, maxs, rT, (ts#ST,LT))              = True"
+"app' (Dup, G, maxs, rT, (ts#ST,LT))              = (1+length ST < maxs)"
+"app' (Dup_x1, G, maxs, rT, (ts1#ts2#ST,LT))      = (2+length ST < maxs)"
+"app' (Dup_x2, G, maxs, rT, (ts1#ts2#ts3#ST,LT))  = (3+length ST < maxs)"
+"app' (Swap, G, maxs, rT, (ts1#ts2#ST,LT))        = True"
+"app' (IAdd, G, maxs, rT, (PrimT Integer#PrimT Integer#ST,LT)) 
+                                                 = True"
+"app' (Ifcmpeq b, G, maxs, rT, (ts#ts'#ST,LT))    = ((\<exists>p. ts = PrimT p \<and> ts' = PrimT p) \<or> 
+                                              (\<exists>r r'. ts = RefT r \<and> ts' = RefT r'))"
+"app' (Goto b, G, maxs, rT, s)                    = True"
+"app' (Return, G, maxs, rT, (T#ST,LT))            = (G \<turnstile> T \<preceq> rT)"
+"app' (Throw, G, maxs, rT, (T#ST,LT))             = (\<exists>r. T = RefT r)"
+"app' (Invoke C mn fpTs, G, maxs, rT, s)          = 
+   (length fpTs < length (fst s) \<and> 
+   (let apTs = rev (take (length fpTs) (fst s));
+        X    = hd (drop (length fpTs) (fst s)) 
+    in  
+        G \<turnstile> X \<preceq> Class C \<and> is_class G C \<and> method (G,C) (mn,fpTs) \<noteq> None \<and> 
+        (\<forall>(aT,fT)\<in>set(zip apTs fpTs). G \<turnstile> aT \<preceq> fT)))"
+
+"app' (i,G,maxs,rT,s)                             = False"
+
+
+
+constdefs
+  xcpt_app :: "instr \<Rightarrow> jvm_prog \<Rightarrow> nat \<Rightarrow> exception_table \<Rightarrow> bool"
+  "xcpt_app i G pc et \<equiv> \<forall>C\<in>set(xcpt_names (i,G,pc,et)). is_class G C"
+
+  app :: "instr => jvm_prog => nat => ty => nat => exception_table => state_type option => bool"
+  "app i G maxs rT pc et s == case s of None => True | Some t => app' (i,G,maxs,rT,t) \<and> xcpt_app i G pc et"
+
+
+lemma 1: "2 < length a ==> (\<exists>l l' l'' ls. a = l#l'#l''#ls)"
+proof (cases a)
+  fix x xs assume "a = x#xs" "2 < length a"
+  thus ?thesis by - (cases xs, simp, cases "tl xs", auto)
+qed auto
+
+lemma 2: "\<not>(2 < length a) ==> a = [] \<or> (\<exists> l. a = [l]) \<or> (\<exists> l l'. a = [l,l'])"
+proof -;
+  assume "\<not>(2 < length a)"
+  hence "length a < (Suc (Suc (Suc 0)))" by simp
+  hence * : "length a = 0 \<or> length a = Suc 0 \<or> length a = Suc (Suc 0)" 
+    by (auto simp add: less_Suc_eq)
+
+  { 
+    fix x 
+    assume "length x = Suc 0"
+    hence "\<exists> l. x = [l]"  by - (cases x, auto)
+  } note 0 = this
+
+  have "length a = Suc (Suc 0) ==> \<exists>l l'. a = [l,l']" by (cases a, auto dest: 0)
+  with * show ?thesis by (auto dest: 0)
+qed
+
+lemmas [simp] = app_def xcpt_app_def
+
+text {* 
+\medskip
+simp rules for @{term app}
+*}
+lemma appNone[simp]: "app i G maxs rT pc et None = True" by simp
+
+
+lemma appLoad[simp]:
+"(app (Load idx) G maxs rT pc et (Some s)) = (\<exists>ST LT. s = (ST,LT) \<and> idx < length LT \<and> LT!idx \<noteq> Err \<and> length ST < maxs)"
+  by (cases s, simp)
+
+lemma appStore[simp]:
+"(app (Store idx) G maxs rT pc et (Some s)) = (\<exists>ts ST LT. s = (ts#ST,LT) \<and> idx < length LT)"
+  by (cases s, cases "2 < length (fst s)", auto dest: 1 2)
+
+lemma appLitPush[simp]:
+"(app (LitPush v) G maxs rT pc et (Some s)) = (\<exists>ST LT. s = (ST,LT) \<and> length ST < maxs \<and> typeof (\<lambda>v. None) v \<noteq> None)"
+  by (cases s, simp)
+
+lemma appGetField[simp]:
+"(app (Getfield F C) G maxs rT pc et (Some s)) = 
+ (\<exists> oT vT ST LT. s = (oT#ST, LT) \<and> is_class G C \<and>  
+  field (G,C) F = Some (C,vT) \<and> G \<turnstile> oT \<preceq> (Class C) \<and> is_class G (Xcpt NullPointer))"
+  by (cases s, cases "2 <length (fst s)", auto dest!: 1 2)
+
+lemma appPutField[simp]:
+"(app (Putfield F C) G maxs rT pc et (Some s)) = 
+ (\<exists> vT vT' oT ST LT. s = (vT#oT#ST, LT) \<and> is_class G C \<and> 
+  field (G,C) F = Some (C, vT') \<and> G \<turnstile> oT \<preceq> (Class C) \<and> G \<turnstile> vT \<preceq> vT' \<and> is_class G (Xcpt NullPointer))"
+  by (cases s, cases "2 <length (fst s)", auto dest!: 1 2)
+
+lemma appNew[simp]:
+  "(app (New C) G maxs rT pc et (Some s)) = 
+  (\<exists>ST LT. s=(ST,LT) \<and> is_class G C \<and> length ST < maxs \<and> is_class G (Xcpt OutOfMemory))"
+  by (cases s, simp)
+
+lemma appCheckcast[simp]: 
+  "(app (Checkcast C) G maxs rT pc et (Some s)) =  
+  (\<exists>rT ST LT. s = (RefT rT#ST,LT) \<and> is_class G C \<and> is_class G (Xcpt ClassCast))"
+  by (cases s, cases "fst s", simp add: app_def) (cases "hd (fst s)", auto)
+
+lemma appPop[simp]: 
+"(app Pop G maxs rT pc et (Some s)) = (\<exists>ts ST LT. s = (ts#ST,LT))"
+  by (cases s, cases "2 <length (fst s)", auto dest: 1 2)
+
+
+lemma appDup[simp]:
+"(app Dup G maxs rT pc et (Some s)) = (\<exists>ts ST LT. s = (ts#ST,LT) \<and> 1+length ST < maxs)" 
+  by (cases s, cases "2 <length (fst s)", auto dest: 1 2)
+
+
+lemma appDup_x1[simp]:
+"(app Dup_x1 G maxs rT pc et (Some s)) = (\<exists>ts1 ts2 ST LT. s = (ts1#ts2#ST,LT) \<and> 2+length ST < maxs)" 
+  by (cases s, cases "2 <length (fst s)", auto dest: 1 2)
+
+
+lemma appDup_x2[simp]:
+"(app Dup_x2 G maxs rT pc et (Some s)) = (\<exists>ts1 ts2 ts3 ST LT. s = (ts1#ts2#ts3#ST,LT) \<and> 3+length ST < maxs)"
+  by (cases s, cases "2 <length (fst s)", auto dest: 1 2)
+
+
+lemma appSwap[simp]:
+"app Swap G maxs rT pc et (Some s) = (\<exists>ts1 ts2 ST LT. s = (ts1#ts2#ST,LT))" 
+  by (cases s, cases "2 <length (fst s)", auto dest: 1 2)
+
+
+lemma appIAdd[simp]:
+"app IAdd G maxs rT pc et (Some s) = (\<exists> ST LT. s = (PrimT Integer#PrimT Integer#ST,LT))"
+  (is "?app s = ?P s")
+proof (cases (open) s)
+  case Pair
+  have "?app (a,b) = ?P (a,b)"
+  proof (cases "a")
+    fix t ts assume a: "a = t#ts"
+    show ?thesis
+    proof (cases t)
+      fix p assume p: "t = PrimT p"
+      show ?thesis
+      proof (cases p)
+        assume ip: "p = Integer"
+        show ?thesis
+        proof (cases ts)
+          fix t' ts' assume t': "ts = t' # ts'"
+          show ?thesis
+          proof (cases t')
+            fix p' assume "t' = PrimT p'"
+            with t' ip p a
+            show ?thesis by - (cases p', auto)
+          qed (auto simp add: a p ip t')
+        qed (auto simp add: a p ip)
+      qed (auto simp add: a p)
+    qed (auto simp add: a)
+  qed auto
+  with Pair show ?thesis by simp
+qed
+
+
+lemma appIfcmpeq[simp]:
+"app (Ifcmpeq b) G maxs rT pc et (Some s) = (\<exists>ts1 ts2 ST LT. s = (ts1#ts2#ST,LT) \<and> 
+ ((\<exists> p. ts1 = PrimT p \<and> ts2 = PrimT p) \<or> (\<exists>r r'. ts1 = RefT r \<and> ts2 = RefT r')))" 
+  by (cases s, cases "2 <length (fst s)", auto dest: 1 2)
+
+
+lemma appReturn[simp]:
+"app Return G maxs rT pc et (Some s) = (\<exists>T ST LT. s = (T#ST,LT) \<and> (G \<turnstile> T \<preceq> rT))" 
+  by (cases s, cases "2 <length (fst s)", auto dest: 1 2)
+
+lemma appGoto[simp]:
+"app (Goto branch) G maxs rT pc et (Some s) = True"
+  by simp
+
+lemma appThrow[simp]:
+  "app Throw G maxs rT pc et (Some s) = 
+  (\<exists>T ST LT r. s=(T#ST,LT) \<and> T = RefT r \<and> (\<forall>C \<in> set (match_any G pc et). is_class G C))"
+  by (cases s, cases "2 < length (fst s)", auto dest: 1 2)
+
+lemma appInvoke[simp]:
+"app (Invoke C mn fpTs) G maxs rT pc et (Some s) = (\<exists>apTs X ST LT mD' rT' b'.
+  s = ((rev apTs) @ (X # ST), LT) \<and> length apTs = length fpTs \<and> is_class G C \<and>
+  G \<turnstile> X \<preceq> Class C \<and> (\<forall>(aT,fT)\<in>set(zip apTs fpTs). G \<turnstile> aT \<preceq> fT) \<and> 
+  method (G,C) (mn,fpTs) = Some (mD', rT', b') \<and> 
+  (\<forall>C \<in> set (match_any G pc et). is_class G C))" (is "?app s = ?P s")
+proof (cases (open) s)
+  case Pair
+  have "?app (a,b) ==> ?P (a,b)"
+  proof -
+    assume app: "?app (a,b)"
+    hence "a = (rev (rev (take (length fpTs) a))) @ (drop (length fpTs) a) \<and> 
+           length fpTs < length a" (is "?a \<and> ?l") 
+      by (auto simp add: app_def)
+    hence "?a \<and> 0 < length (drop (length fpTs) a)" (is "?a \<and> ?l") 
+      by auto
+    hence "?a \<and> ?l \<and> length (rev (take (length fpTs) a)) = length fpTs" 
+      by (auto simp add: min_def)
+    hence "\<exists>apTs ST. a = rev apTs @ ST \<and> length apTs = length fpTs \<and> 0 < length ST" 
+      by blast
+    hence "\<exists>apTs ST. a = rev apTs @ ST \<and> length apTs = length fpTs \<and> ST \<noteq> []" 
+      by blast
+    hence "\<exists>apTs ST. a = rev apTs @ ST \<and> length apTs = length fpTs \<and> 
+           (\<exists>X ST'. ST = X#ST')" 
+      by (simp add: neq_Nil_conv)
+    hence "\<exists>apTs X ST. a = rev apTs @ X # ST \<and> length apTs = length fpTs" 
+      by blast
+    with app
+    show ?thesis by (unfold app_def, clarsimp) blast
+  qed
+  with Pair 
+  have "?app s ==> ?P s" by simp
+  moreover
+  have "?P s \<Longrightarrow> ?app s" by (unfold app_def) clarsimp
+  ultimately
+  show ?thesis by blast
+qed 
+
+lemma effNone: 
+  "(pc', s') \<in> set (eff i G pc et None) \<Longrightarrow> s' = None"
+  by (auto simp add: eff_def xcpt_eff_def norm_eff_def)
+
+lemmas [simp del] = app_def xcpt_app_def
+
+end
