src/HOL/MicroJava/BV/EffectMono.thy
@@ -1,12 +1,12 @@
-(*  Title:      HOL/MicroJava/BV/StepMono.thy
+(*  Title:      HOL/MicroJava/BV/EffMono.thy
     ID:         $Id$
     Author:     Gerwin Klein
     Copyright   2000 Technische Universitaet Muenchen
 *)
 
-header {* Monotonicity of step and app *}
+header {* Monotonicity of eff and app *}
 
-theory StepMono = Step:
+theory EffectMono = Effect:
 
 
 lemma PrimT_PrimT: "(G \<turnstile> xb \<preceq> PrimT p) = (xb = PrimT p)"
@@ -14,52 +14,52 @@ lemma PrimT_PrimT: "(G \<turnstile> xb \<preceq> PrimT p) = (xb = PrimT p)"
 
 
 lemma sup_loc_some [rule_format]:
-"\<forall> y n. (G \<turnstile> b <=l y) --> n < length y --> y!n = OK t -->
+"\<forall>y n. (G \<turnstile> b <=l y) --> n < length y --> y!n = OK t --> 
   (\<exists>t. b!n = OK t \<and> (G \<turnstile> (b!n) <=o (y!n)))" (is "?P b")
 proof (induct (open) ?P b)
   show "?P []" by simp
 
   case Cons
-  show "?P (a#list)"
+  show "?P (a#list)" 
   proof (clarsimp simp add: list_all2_Cons1 sup_loc_def Listn.le_def lesub_def)
     fix z zs n
-    assume * :
-      "G \<turnstile> a <=o z" "list_all2 (sup_ty_opt G) list zs"
+    assume * : 
+      "G \<turnstile> a <=o z" "list_all2 (sup_ty_opt G) list zs" 
       "n < Suc (length list)" "(z # zs) ! n = OK t"
 
-    show "(\<exists>t. (a # list) ! n = OK t) \<and> G \<turnstile>(a # list) ! n <=o OK t"
-    proof (cases n)
+    show "(\<exists>t. (a # list) ! n = OK t) \<and> G \<turnstile>(a # list) ! n <=o OK t" 
+    proof (cases n) 
       case 0
       with * show ?thesis by (simp add: sup_ty_opt_OK)
     next
       case Suc
       with Cons *
-      show ?thesis by (simp add: sup_loc_def Listn.le_def lesub_def)
+      show ?thesis by (simp add: sup_loc_def Listn.le_def lesub_def) 
     qed
-  qed
+  qed 
 qed
-
+   
 
 lemma all_widen_is_sup_loc:
-"\<forall>b. length a = length b -->
-     (\<forall>x\<in>set (zip a b). x \<in> widen G) = (G \<turnstile> (map OK a) <=l (map OK b))"
+"\<forall>b. length a = length b --> 
+     (\<forall>x\<in>set (zip a b). x \<in> widen G) = (G \<turnstile> (map OK a) <=l (map OK b))" 
  (is "\<forall>b. length a = length b --> ?Q a b" is "?P a")
 proof (induct "a")
   show "?P []" by simp
 
   fix l ls assume Cons: "?P ls"
 
-  show "?P (l#ls)"
+  show "?P (l#ls)" 
   proof (intro allI impI)
-    fix b
-    assume "length (l # ls) = length (b::ty list)"
+    fix b 
+    assume "length (l # ls) = length (b::ty list)" 
     with Cons
     show "?Q (l # ls) b" by - (cases b, auto)
   qed
 qed
+ 
 
-
-lemma append_length_n [rule_format]:
+lemma append_length_n [rule_format]: 
 "\<forall>n. n \<le> length x --> (\<exists>a b. x = a@b \<and> length a = n)" (is "?P x")
 proof (induct (open) ?P x)
   show "?P []" by simp
@@ -71,13 +71,12 @@ proof (induct (open) ?P x)
     fix n
     assume l: "n \<le> length (l # ls)"
 
-    show "\<exists>a b. l # ls = a @ b \<and> length a = n"
+    show "\<exists>a b. l # ls = a @ b \<and> length a = n" 
     proof (cases n)
       assume "n=0" thus ?thesis by simp
     next
-      fix "n'" assume s: "n = Suc n'"
-      with l
-      have  "n' \<le> length ls" by simp
+      fix n' assume s: "n = Suc n'"
+      with l have  "n' \<le> length ls" by simp
       hence "\<exists>a b. ls = a @ b \<and> length a = n'" by (rule Cons [rule_format])
       then obtain a b where "ls = a @ b" "length a = n'" by rules
       with s have "l # ls = (l#a) @ b \<and> length (l#a) = n" by simp
@@ -86,9 +85,8 @@ proof (induct (open) ?P x)
   qed
 qed
 
-
 lemma rev_append_cons:
-"[|n < length x|] ==> \<exists>a b c. x = (rev a) @ b # c \<and> length a = n"
+"n < length x ==> \<exists>a b c. x = (rev a) @ b # c \<and> length a = n"
 proof -
   assume n: "n < length x"
   hence "n \<le> length x" by simp
@@ -100,54 +98,60 @@ proof -
   thus ?thesis by blast
 qed
 
+lemma sup_loc_length_map:
+  "G \<turnstile> map f a <=l map g b \<Longrightarrow> length a = length b"
+proof -
+  assume "G \<turnstile> map f a <=l map g b"
+  hence "length (map f a) = length (map g b)" by (rule sup_loc_length)
+  thus ?thesis by simp
+qed
+
 lemmas [iff] = not_Err_eq
 
-lemma app_mono:
-"[|G \<turnstile> s <=' s'; app i G m rT s'|] ==> app i G m rT s"
+lemma app_mono: 
+"[|G \<turnstile> s <=' s'; app i G m rT pc et s'|] ==> app i G m rT pc et s"
 proof -
 
   { fix s1 s2
     assume G:   "G \<turnstile> s2 <=s s1"
-    assume app: "app i G m rT (Some s1)"
+    assume app: "app i G m rT pc et (Some s1)"
 
-    have "app i G m rT (Some s2)"
+    note [simp] = sup_loc_length sup_loc_length_map
+
+    have "app i G m rT pc et (Some s2)"
     proof (cases (open) i)
       case Load
-
+    
       from G Load app
       have "G \<turnstile> snd s2 <=l snd s1" by (auto simp add: sup_state_conv)
-
-      with G Load app
-      show ?thesis
-        by (auto dest: sup_loc_some)
+      
+      with G Load app show ?thesis 
+        by (cases s2) (auto simp add: sup_state_conv dest: sup_loc_some)
     next
       case Store
-      with G app
-      show ?thesis
-        by (cases s2) (auto simp add: map_eq_Cons sup_loc_Cons2 sup_loc_length sup_state_conv)
+      with G app show ?thesis
+        by (cases s2, auto simp add: map_eq_Cons sup_loc_Cons2 sup_state_conv)
     next
       case LitPush
-      with G app
-      show ?thesis by simp
+      with G app show ?thesis by (cases s2, auto simp add: sup_state_conv)
     next
       case New
-      with G app
-      show ?thesis by simp
+      with G app show ?thesis by (cases s2, auto simp add: sup_state_conv)
     next
       case Getfield
-      with app G
-      show ?thesis
-        by (cases s2) (auto simp add: sup_state_Cons2, rule widen_trans)
+      with app G show ?thesis
+        by (cases s2) (clarsimp simp add: sup_state_Cons2, rule widen_trans) 
     next
       case Putfield
-
-      with app
+      
+      with app 
       obtain vT oT ST LT b
         where s1: "s1 = (vT # oT # ST, LT)" and
-                  "field (G, cname) vname = Some (cname, b)"
+                  "field (G, cname) vname = Some (cname, b)" 
                   "is_class G cname" and
               oT: "G\<turnstile> oT\<preceq> (Class cname)" and
-              vT: "G\<turnstile> vT\<preceq> b"
+              vT: "G\<turnstile> vT\<preceq> b" and
+              xc: "is_class G (Xcpt NullPointer)"
         by force
       moreover
       from s1 G
@@ -155,7 +159,7 @@ proof -
         where s2:  "s2 = (vT' # oT' # ST', LT')" and
               oT': "G\<turnstile> oT' \<preceq> oT" and
               vT': "G\<turnstile> vT' \<preceq> vT"
-        by (cases s2) (auto simp add: sup_state_Cons2)
+        by - (cases s2, simp add: sup_state_Cons2, elim exE conjE, simp, rule that)
       moreover
       from vT' vT
       have "G \<turnstile> vT' \<preceq> b" by (rule widen_trans)
@@ -163,63 +167,52 @@ proof -
       from oT' oT
       have "G\<turnstile> oT' \<preceq> (Class cname)" by (rule widen_trans)
       ultimately
-      show ?thesis
-        by (auto simp add: Putfield)
+      show ?thesis by (auto simp add: Putfield xc)
     next
       case Checkcast
-      with app G
-      show ?thesis
-        by (cases s2) (auto intro!: widen_RefT2 simp add: sup_state_Cons2)
+      with app G show ?thesis 
+        by (cases s2, auto intro!: widen_RefT2 simp add: sup_state_Cons2)
     next
       case Return
-      with app G
-      show ?thesis
+      with app G show ?thesis
         by (cases s2) (auto simp add: sup_state_Cons2, rule widen_trans)
     next
       case Pop
-      with app G
-      show ?thesis
-        by (cases s2) (auto simp add: sup_state_Cons2)
+      with app G show ?thesis
+        by (cases s2, clarsimp simp add: sup_state_Cons2)
     next
       case Dup
-      with app G
-      show ?thesis
-        by (cases s2) (clarsimp simp add: sup_state_Cons2,
-              auto dest: sup_state_length)
+      with app G show ?thesis
+        by (cases s2, clarsimp simp add: sup_state_Cons2,
+            auto dest: sup_state_length)
     next
       case Dup_x1
-      with app G
-      show ?thesis
-        by (cases s2) (clarsimp simp add: sup_state_Cons2,
-              auto dest: sup_state_length)
+      with app G show ?thesis
+        by (cases s2, clarsimp simp add: sup_state_Cons2, 
+            auto dest: sup_state_length)
     next
       case Dup_x2
-      with app G
-      show ?thesis
-        by (cases s2) (clarsimp simp add: sup_state_Cons2,
-              auto dest: sup_state_length)
+      with app G show ?thesis
+        by (cases s2, clarsimp simp add: sup_state_Cons2,
+            auto dest: sup_state_length)
     next
       case Swap
-      with app G
-      show ?thesis
-        by (cases s2) (clarsimp simp add: sup_state_Cons2)
+      with app G show ?thesis
+        by (cases s2, clarsimp simp add: sup_state_Cons2)
     next
       case IAdd
-      with app G
-      show ?thesis
-        by (cases s2) (auto simp add: sup_state_Cons2 PrimT_PrimT)
+      with app G show ?thesis
+        by (cases s2, auto simp add: sup_state_Cons2 PrimT_PrimT)
     next
-      case Goto
-      with app
-      show ?thesis by simp
+      case Goto 
+      with app show ?thesis by simp
     next
       case Ifcmpeq
-      with app G
-      show ?thesis
-        by (cases s2) (auto simp add: sup_state_Cons2 PrimT_PrimT widen_RefT2)
+      with app G show ?thesis
+        by (cases s2, auto simp add: sup_state_Cons2 PrimT_PrimT widen_RefT2)
     next
       case Invoke
-
+      
       with app
       obtain apTs X ST LT mD' rT' b' where
         s1: "s1 = (rev apTs @ X # ST, LT)" and
@@ -227,41 +220,42 @@ proof -
         c:  "is_class G cname" and
         C:  "G \<turnstile> X \<preceq> Class cname" and
         w:  "\<forall>x \<in> set (zip apTs list). x \<in> widen G" and
-        m:  "method (G, cname) (mname, list) = Some (mD', rT', b')"
-        by (simp del: not_None_eq) blast+
+        m:  "method (G, cname) (mname, list) = Some (mD', rT', b')" and
+        x:  "\<forall>C \<in> set (match_any G pc et). is_class G C"
+        by (simp del: not_None_eq, elim exE conjE) (rule that)
 
       obtain apTs' X' ST' LT' where
         s2: "s2 = (rev apTs' @ X' # ST', LT')" and
         l': "length apTs' = length list"
       proof -
-        from l s1 G
-        have "length list < length (fst s2)"
+        from l s1 G 
+        have "length list < length (fst s2)" 
           by simp
         hence "\<exists>a b c. (fst s2) = rev a @ b # c \<and> length a = length list"
           by (rule rev_append_cons [rule_format])
         thus ?thesis
-          by - (cases s2, elim exE conjE, simp, rule that)
+          by -  (cases s2, elim exE conjE, simp, rule that) 
       qed
 
       from l l'
       have "length (rev apTs') = length (rev apTs)" by simp
-
-      from this s1 s2 G
+    
+      from this s1 s2 G 
       obtain
         G': "G \<turnstile> (apTs',LT') <=s (apTs,LT)" and
         X : "G \<turnstile>  X' \<preceq> X" and "G \<turnstile> (ST',LT') <=s (ST,LT)"
         by (simp add: sup_state_rev_fst sup_state_append_fst sup_state_Cons1)
-
+        
       with C
       have C': "G \<turnstile> X' \<preceq> Class cname"
         by - (rule widen_trans, auto)
-
+    
       from G'
       have "G \<turnstile> map OK apTs' <=l map OK apTs"
         by (simp add: sup_state_conv)
       also
       from l w
-      have "G \<turnstile> map OK apTs <=l map OK list"
+      have "G \<turnstile> map OK apTs <=l map OK list" 
         by (simp add: all_widen_is_sup_loc)
       finally
       have "G \<turnstile> map OK apTs' <=l map OK list" .
@@ -270,94 +264,88 @@ proof -
       have w': "\<forall>x \<in> set (zip apTs' list). x \<in> widen G"
         by (simp add: all_widen_is_sup_loc)
 
-      from Invoke s2 l' w' C' m c
+      from Invoke s2 l' w' C' m c x
       show ?thesis
         by (simp del: split_paired_Ex) blast
+    next
+      case Throw
+      with app G show ?thesis
+        by (cases s2, clarsimp simp add: sup_state_Cons2 widen_RefT2)
     qed
   } note this [simp]
 
-  assume "G \<turnstile> s <=' s'" "app i G m rT s'"
-
-  thus ?thesis
-    by - (cases s, cases s', auto)
+  assume "G \<turnstile> s <=' s'" "app i G m rT pc et s'"
+  thus ?thesis by (cases s, cases s', auto)
 qed
-
+    
 lemmas [simp del] = split_paired_Ex
-lemmas [simp] = step_def
 
-lemma step_mono_Some:
-"[| app i G m rT (Some s2); G \<turnstile> s1 <=s s2 |] ==>
-  G \<turnstile> the (step i G (Some s1)) <=s the (step i G (Some s2))"
+lemma eff'_mono:
+"[| app i G m rT pc et (Some s2); G \<turnstile> s1 <=s s2 |] ==>
+  G \<turnstile> eff' (i,G,s1) <=s eff' (i,G,s2)"
 proof (cases s1, cases s2)
   fix a1 b1 a2 b2
   assume s: "s1 = (a1,b1)" "s2 = (a2,b2)"
-  assume app2: "app i G m rT (Some s2)"
+  assume app2: "app i G m rT pc et (Some s2)"
   assume G: "G \<turnstile> s1 <=s s2"
+  
+  note [simp] = eff_def
 
-  hence "G \<turnstile> Some s1 <=' Some s2"
-    by simp
+  hence "G \<turnstile> (Some s1) <=' (Some s2)" by simp
   from this app2
-  have app1: "app i G m rT (Some s1)" by (rule app_mono)
+  have app1: "app i G m rT pc et (Some s1)" by (rule app_mono)
 
-  have "step i G (Some s1) \<noteq> None \<and> step i G (Some s2) \<noteq> None"
-    by simp
-  then
-  obtain a1' b1' a2' b2'
-    where step: "step i G (Some s1) = Some (a1',b1')"
-                "step i G (Some s2) = Some (a2',b2')"
-    by (auto simp del: step_def simp add: s)
-
-  have "G \<turnstile> (a1',b1') <=s (a2',b2')"
+  show ?thesis
   proof (cases (open) i)
     case Load
 
     with s app1
     obtain y where
-       y:  "nat < length b1" "b1 ! nat = OK y" by auto
+       y:  "nat < length b1" "b1 ! nat = OK y" by clarsimp
 
     from Load s app2
     obtain y' where
-       y': "nat < length b2" "b2 ! nat = OK y'" by auto
+       y': "nat < length b2" "b2 ! nat = OK y'" by clarsimp
 
-    from G s
+    from G s 
     have "G \<turnstile> b1 <=l b2" by (simp add: sup_state_conv)
 
     with y y'
-    have "G \<turnstile> y \<preceq> y'"
-      by (auto dest: sup_loc_some)
-
-    with Load G y y' s step app1 app2
-    show ?thesis by (auto simp add: sup_state_conv)
+    have "G \<turnstile> y \<preceq> y'" 
+      by - (drule sup_loc_some, simp+)
+    
+    with Load G y y' s app1 app2 
+    show ?thesis by (clarsimp simp add: sup_state_conv)
   next
     case Store
-    with G s step app1 app2
+    with G s app1 app2
     show ?thesis
-      by (auto simp add: sup_state_conv sup_loc_update)
+      by (clarsimp simp add: sup_state_conv sup_loc_update)
   next
     case LitPush
-    with G s step app1 app2
+    with G s app1 app2
     show ?thesis
-      by (auto simp add: sup_state_Cons1)
+      by (clarsimp simp add: sup_state_Cons1)
   next
     case New
-    with G s step app1 app2
+    with G s app1 app2
     show ?thesis
-      by (auto simp add: sup_state_Cons1)
+      by (clarsimp simp add: sup_state_Cons1)
   next
     case Getfield
-    with G s step app1 app2
+    with G s app1 app2
     show ?thesis
-      by (auto simp add: sup_state_Cons1)
+      by (clarsimp simp add: sup_state_Cons1)
   next
     case Putfield
-    with G s step app1 app2
+    with G s app1 app2
     show ?thesis
-      by (auto simp add: sup_state_Cons1)
+      by (clarsimp simp add: sup_state_Cons1)
   next
     case Checkcast
-    with G s step app1 app2
+    with G s app1 app2
     show ?thesis
-      by (auto simp add: sup_state_Cons1)
+      by (clarsimp simp add: sup_state_Cons1)
   next
     case Invoke
 
@@ -365,89 +353,89 @@ proof (cases s1, cases s2)
     obtain a X ST where
       s1: "s1 = (a @ X # ST, b1)" and
       l:  "length a = length list"
-      by auto
+      by (simp, elim exE conjE, simp)
 
     from Invoke s app2
     obtain a' X' ST' where
       s2: "s2 = (a' @ X' # ST', b2)" and
       l': "length a' = length list"
-      by auto
+      by (simp, elim exE conjE, simp)
 
     from l l'
     have lr: "length a = length a'" by simp
-
-    from lr G s s1 s2
+      
+    from lr G s s1 s2 
     have "G \<turnstile> (ST, b1) <=s (ST', b2)"
       by (simp add: sup_state_append_fst sup_state_Cons1)
-
+    
     moreover
 
-    from Invoke G s step app1 app2
-    have "b1 = b1' \<and> b2 = b2'" by simp
+    obtain b1' b2' where eff':
+      "b1' = snd (eff' (i,G,s1))" 
+      "b2' = snd (eff' (i,G,s2))" by simp
 
-    ultimately
+    from Invoke G s eff' app1 app2
+    obtain "b1 = b1'" "b2 = b2'" by simp
+
+    ultimately 
 
     have "G \<turnstile> (ST, b1') <=s (ST', b2')" by simp
 
-    with Invoke G s step app1 app2 s1 s2 l l'
-    show ?thesis
-      by (auto simp add: sup_state_conv)
+    with Invoke G s app1 app2 eff' s1 s2 l l'
+    show ?thesis 
+      by (clarsimp simp add: sup_state_conv)
   next
-    case Return
-    with G step
+    case Return 
+    with G
     show ?thesis
       by simp
   next
     case Pop
-    with G s step app1 app2
+    with G s app1 app2
     show ?thesis
-      by (auto simp add: sup_state_Cons1)
+      by (clarsimp simp add: sup_state_Cons1)
   next
     case Dup
-    with G s step app1 app2
+    with G s app1 app2
     show ?thesis
-      by (auto simp add: sup_state_Cons1)
+      by (clarsimp simp add: sup_state_Cons1)
   next
     case Dup_x1
-    with G s step app1 app2
+    with G s app1 app2
     show ?thesis
-      by (auto simp add: sup_state_Cons1)
-  next
+      by (clarsimp simp add: sup_state_Cons1)
+  next 
     case Dup_x2
-    with G s step app1 app2
+    with G s app1 app2
     show ?thesis
-      by (auto simp add: sup_state_Cons1)
+      by (clarsimp simp add: sup_state_Cons1)
   next
     case Swap
-    with G s step app1 app2
+    with G s app1 app2
     show ?thesis
-      by (auto simp add: sup_state_Cons1)
+      by (clarsimp simp add: sup_state_Cons1)
   next
     case IAdd
-    with G s step app1 app2
+    with G s app1 app2
     show ?thesis
-      by (auto simp add: sup_state_Cons1)
+      by (clarsimp simp add: sup_state_Cons1)
   next
     case Goto
-    with G s step app1 app2
+    with G s app1 app2
     show ?thesis by simp
   next
     case Ifcmpeq
-    with G s step app1 app2
+    with G s app1 app2
     show ?thesis
-      by (auto simp add: sup_state_Cons1)
+      by (clarsimp simp add: sup_state_Cons1)
+  next 
+    case Throw
+    with G
+    show ?thesis
+      by simp
   qed
-
-  with step
-  show ?thesis by auto
 qed
 
-lemma step_mono:
-  "[| app i G m rT s2; G \<turnstile> s1 <=' s2 |] ==>
-  G \<turnstile> step i G s1 <=' step i G s2"
-  by (cases s1, cases s2, auto dest: step_mono_Some)
-
-lemmas [simp del] = step_def
 lemmas [iff del] = not_Err_eq
 
 end
