src/HOL/MicroJava/BV/LBVCorrect.thy
@@ -6,72 +6,75 @@
 
 header {* Correctness of the LBV *}
 
+(* This theory is currently broken. The port to exceptions
+  didn't make it into the Isabelle 2001 release. It is included for 
+  documentation only. See Isabelle 99-2 for a working copy of this
+  theory. *)
+
+
 theory LBVCorrect = BVSpec + LBVSpec:
 
 lemmas [simp del] = split_paired_Ex split_paired_All
 
 constdefs
-fits :: "[method_type,instr list,jvm_prog,ty,state_type option,nat,certificate] => bool"
-"fits phi is G rT s0 maxs cert == 
+fits :: "[method_type,instr list,jvm_prog,ty,state_type option,nat,nat,exception_table,certificate] => bool"
+"fits phi is G rT s0 maxs maxr et cert == 
   (\<forall>pc s1. pc < length is -->
-    (wtl_inst_list (take pc is) G rT cert maxs (length is) 0 s0 = OK s1 -->
+    (wtl_inst_list (take pc is) G rT cert maxs maxr (length is) et 0 s0 = OK s1 -->
     (case cert!pc of None   => phi!pc = s1
                    | Some t => phi!pc = Some t)))"
 
 constdefs
-make_phi :: "[instr list,jvm_prog,ty,state_type option,nat,certificate] => method_type"
-"make_phi is G rT s0 maxs cert == 
+make_phi :: "[instr list,jvm_prog,ty,state_type option,nat,nat,exception_table,certificate] => method_type"
+"make_phi is G rT s0 maxs maxr et cert == 
    map (\<lambda>pc. case cert!pc of 
-               None   => ok_val (wtl_inst_list (take pc is) G rT cert maxs (length is) 0 s0) 
+               None   => ok_val (wtl_inst_list (take pc is) G rT cert maxs maxr (length is) et 0 s0) 
              | Some t => Some t) [0..length is(]"
 
 
 lemma fitsD_None:
-  "[|fits phi is G rT s0 mxs cert; pc < length is;
-    wtl_inst_list (take pc is) G rT cert mxs (length is) 0 s0 = OK s1; 
+  "[|fits phi is G rT s0 mxs mxr et cert; pc < length is;
+    wtl_inst_list (take pc is) G rT cert mxs mxr (length is) et 0 s0 = OK s1; 
     cert ! pc = None|] ==> phi!pc = s1"
   by (auto simp add: fits_def)
 
 lemma fitsD_Some:
-  "[|fits phi is G rT s0 mxs cert; pc < length is;
-    wtl_inst_list (take pc is) G rT cert mxs (length is) 0 s0 = OK s1; 
+  "[|fits phi is G rT s0 mxs mxr et cert; pc < length is;
+    wtl_inst_list (take pc is) G rT cert mxs mxr (length is) et 0 s0 = OK s1; 
     cert ! pc = Some t|] ==> phi!pc = Some t"
   by (auto simp add: fits_def)
 
 lemma make_phi_Some:
   "[| pc < length is; cert!pc = Some t |] ==> 
-  make_phi is G rT s0 mxs cert ! pc = Some t"
+  make_phi is G rT s0 mxs mxr et cert ! pc = Some t"
   by (simp add: make_phi_def)
 
 lemma make_phi_None:
   "[| pc < length is; cert!pc = None |] ==> 
-  make_phi is G rT s0 mxs cert ! pc = 
-  ok_val (wtl_inst_list (take pc is) G rT cert mxs (length is) 0 s0)"
+  make_phi is G rT s0 mxs mxr et cert ! pc = 
+  ok_val (wtl_inst_list (take pc is) G rT cert mxs mxr (length is) et 0 s0)"
   by (simp add: make_phi_def)
 
 lemma exists_phi:
-  "\<exists>phi. fits phi is G rT s0 mxs cert"  
+  "\<exists>phi. fits phi is G rT s0 mxs mxr et cert"  
 proof - 
-  have "fits (make_phi is G rT s0 mxs cert) is G rT s0 mxs cert"
+  have "fits (make_phi is G rT s0 mxs mxr et cert) is G rT s0 mxs mxr et cert"
     by (auto simp add: fits_def make_phi_Some make_phi_None 
              split: option.splits) 
-
-  thus ?thesis
-    by blast
+  thus ?thesis by fast
 qed
   
 lemma fits_lemma1:
-  "[| wtl_inst_list is G rT cert mxs (length is) 0 s = OK s'; fits phi is G rT s mxs cert |]
+  "[| wtl_inst_list is G rT cert mxs mxr (length is) et 0 s = OK s'; fits phi is G rT s mxs mxr et cert |]
   ==> \<forall>pc t. pc < length is --> cert!pc = Some t --> phi!pc = Some t"
 proof (intro strip)
   fix pc t 
-  assume "wtl_inst_list is G rT cert mxs (length is) 0 s = OK s'"
-  then 
-  obtain s'' where
-    "wtl_inst_list (take pc is) G rT cert mxs (length is) 0 s = OK s''"
+  assume "wtl_inst_list is G rT cert mxs mxr (length is) et 0 s = OK s'"
+  then obtain s'' where
+    "wtl_inst_list (take pc is) G rT cert mxs mxr (length is) et 0 s = OK s''"
     by (blast dest: wtl_take)
   moreover
-  assume "fits phi is G rT s mxs cert" 
+  assume "fits phi is G rT s mxs mxr et cert" 
          "pc < length is" 
          "cert ! pc = Some t"
   ultimately
@@ -80,42 +83,42 @@ qed
 
 
 lemma wtl_suc_pc:
- "[| wtl_inst_list is G rT cert mxs (length is) 0 s \<noteq> Err;
-     wtl_inst_list (take pc is) G rT cert mxs (length is) 0 s = OK s';
-     wtl_cert (is!pc) G rT s' cert mxs (length is) pc = OK s'';
-     fits phi is G rT s mxs cert; Suc pc < length is |] ==>
+ "[| wtl_inst_list is G rT cert mxs mxr (length is) et 0 s \<noteq> Err;
+     wtl_inst_list (take pc is) G rT cert mxs mxr (length is) et 0 s = OK s';
+     wtl_cert (is!pc) G rT s' cert mxs mxr (length is) et pc = OK s'';
+     fits phi is G rT s mxs mxr et cert; Suc pc < length is |] ==>
   G \<turnstile> s'' <=' phi ! Suc pc"
 proof -
   
-  assume all:  "wtl_inst_list is G rT cert mxs (length is) 0 s \<noteq> Err"
-  assume fits: "fits phi is G rT s mxs cert"
+  assume all:  "wtl_inst_list is G rT cert mxs mxr (length is) et 0 s \<noteq> Err"
+  assume fits: "fits phi is G rT s mxs mxr et cert"
 
-  assume wtl:  "wtl_inst_list (take pc is) G rT cert mxs (length is) 0 s = OK s'" and
-         wtc:  "wtl_cert (is!pc) G rT s' cert mxs (length is) pc = OK s''" and
+  assume wtl:  "wtl_inst_list (take pc is) G rT cert mxs mxr (length is) et 0 s = OK s'" and
+         wtc:  "wtl_cert (is!pc) G rT s' cert mxs mxr (length is) et pc = OK s''" and
          pc:   "Suc pc < length is"
 
-  hence wts: "wtl_inst_list (take (Suc pc) is) G rT cert mxs (length is) 0 s = OK s''"
+  hence wts: 
+    "wtl_inst_list (take (Suc pc) is) G rT cert mxs mxr (length is) et 0 s = OK s''"
     by (rule wtl_Suc)
 
   from all
   have app: 
-  "wtl_inst_list (take (Suc pc) is@drop (Suc pc) is) G rT cert mxs (length is) 0 s \<noteq> Err"
+  "wtl_inst_list (take (Suc pc) is@drop (Suc pc) is) G rT cert mxs mxr (length is) et 0 s \<noteq> Err"
     by simp
 
   from pc 
   have "0 < length (drop (Suc pc) is)" 
     by simp
-  then 
-  obtain l ls where
+  then obtain l ls where
     "drop (Suc pc) is = l#ls"
     by (auto simp add: neq_Nil_conv simp del: length_drop)
   with app wts pc
   obtain x where 
-    "wtl_cert l G rT s'' cert mxs (length is) (Suc pc) = OK x"
+    "wtl_cert l G rT s'' cert mxs mxr (length is) et (Suc pc) = OK x"
     by (auto simp add: wtl_append min_def simp del: append_take_drop_id)
 
   hence c1: "!!t. cert!Suc pc = Some t ==> G \<turnstile> s'' <=' cert!Suc pc"
-    by (simp add: wtl_cert_def split: if_splits)
+    by (simp add: wtl_cert_def split: split_if_asm)
   moreover
   from fits pc wts
   have c2: "!!t. cert!Suc pc = Some t ==> phi!Suc pc = cert!Suc pc"
@@ -125,110 +128,85 @@ proof -
   have c3: "cert!Suc pc = None ==> phi!Suc pc = s''"
     by (rule fitsD_None)
   ultimately
-
-  show ?thesis 
-    by - (cases "cert ! Suc pc", auto)
+  show ?thesis by (cases "cert!Suc pc", auto)
 qed
 
 
 lemma wtl_fits_wt:
-  "[| wtl_inst_list is G rT cert mxs (length is) 0 s \<noteq> Err; 
-      fits phi is G rT s mxs cert; pc < length is |] ==>
-   wt_instr (is!pc) G rT phi mxs (length is) pc"
+  "[| wtl_inst_list is G rT cert mxs mxr (length is) et 0 s \<noteq> Err; 
+      fits phi is G rT s mxs mxr et cert; pc < length is |] ==>
+   wt_instr (is!pc) G rT phi mxs (length is) et pc"
 proof -
-
-  assume fits: "fits phi is G rT s mxs cert"
-
+  assume fits: "fits phi is G rT s mxs mxr et cert"
   assume pc:  "pc < length is" and
-         wtl: "wtl_inst_list is G rT cert mxs (length is) 0 s \<noteq> Err"
-        
-  then
-  obtain s' s'' where
-    w: "wtl_inst_list (take pc is) G rT cert mxs (length is) 0 s = OK s'" and
-    c: "wtl_cert (is!pc) G rT s' cert mxs (length is) pc = OK s''"
+         wtl: "wtl_inst_list is G rT cert mxs mxr (length is) et 0 s \<noteq> Err"        
+  then obtain s' s'' where
+    w: "wtl_inst_list (take pc is) G rT cert mxs mxr (length is) et 0 s = OK s'" and
+    c: "wtl_cert (is!pc) G rT s' cert mxs mxr (length is) et pc = OK s''"
     by - (drule wtl_all, auto)
 
-  from fits wtl pc
-  have cert_Some: 
+  from fits wtl pc have cert_Some: 
     "!!t pc. [| pc < length is; cert!pc = Some t |] ==> phi!pc = Some t"
     by (auto dest: fits_lemma1)
   
-  from fits wtl pc
-  have cert_None: "cert!pc = None ==> phi!pc = s'"
+  from fits wtl pc have cert_None: "cert!pc = None ==> phi!pc = s'"
     by - (drule fitsD_None)
   
   from pc c cert_None cert_Some
-  have wti: "wtl_inst (is ! pc) G rT (phi!pc) cert mxs (length is) pc = OK s''"
-    by (auto simp add: wtl_cert_def split: if_splits option.splits)
+  have wti: "wtl_inst (is ! pc) G rT (phi!pc) cert mxs mxr (length is) et pc = OK s''"
+    by (auto simp add: wtl_cert_def split: split_if_asm option.splits)
 
-  { fix pc'
-    assume pc': "pc' \<in> set (succs (is!pc) pc)"
+  -- "we now must show that @{text wt_instr} holds; the definition 
+      of @{text wt_instr} is: @{thm [display] wt_instr_def[no_vars]}"
 
-    with wti
-    have less: "pc' < length is"  
-      by (simp add: wtl_inst_OK)
+  { fix pc' r
+    assume pc': "(pc',r) \<in> set (eff (is!pc) G pc et (phi!pc))"
 
-    have "G \<turnstile> step (is!pc) G (phi!pc) <=' phi ! pc'" 
+    with wti have less: "pc' < length is" by (simp add: wtl_inst_OK) blast
+
+    have "G \<turnstile> r <=' phi ! pc'" 
     proof (cases "pc' = Suc pc")
       case False          
       with wti pc'
-      have G: "G \<turnstile> step (is ! pc) G (phi ! pc) <=' cert ! pc'" 
-        by (simp add: wtl_inst_OK)
-
-      hence "cert!pc' = None ==> step (is ! pc) G (phi ! pc) = None"
-        by simp
-      hence "cert!pc' = None ==> ?thesis"
-        by simp
-
-      moreover
-      { fix t
-        assume "cert!pc' = Some t"
-        with less
-        have "phi!pc' = cert!pc'"
-          by (simp add: cert_Some)
-        with G
-        have ?thesis
-          by simp
+      have G: "G \<turnstile> r <=' cert ! pc'" by (simp add: wtl_inst_OK) blast
+      hence "cert!pc' = None ==> r = None" by simp
+      hence "cert!pc' = None ==> ?thesis" by simp
+      moreover {
+        fix t assume "cert!pc' = Some t"
+        with less have "phi!pc' = cert!pc'" by (simp add: cert_Some)
+        with G have ?thesis by simp
       }
-
-      ultimately
-      show ?thesis by blast      
+      ultimately show ?thesis by blast      
     next
       case True
       with pc' wti
-      have "step (is ! pc) G (phi ! pc) = s''"  
-        by (simp add: wtl_inst_OK)
+      have "G \<turnstile> r <=' s''"  sorry
       also
-      from w c fits pc wtl 
-      have "Suc pc < length is ==> G \<turnstile> s'' <=' phi ! Suc pc"
-        by - (drule wtl_suc_pc)
+      from wtl w fits c pc 
+      have "Suc pc < length is ==> G \<turnstile> s'' <=' phi ! Suc pc" 
+        by - (rule wtl_suc_pc)
       with True less
-      have "G \<turnstile> s'' <=' phi ! Suc pc" 
-        by blast
-      finally
-      show ?thesis 
-        by (simp add: True)
+      have "G \<turnstile> s'' <=' phi ! Suc pc" by blast
+      finally show ?thesis by (simp add: True)
     qed
-  }
-  
-  with wti
-  show ?thesis
+  }  
+  with wti show ?thesis
     by (auto simp add: wtl_inst_OK wt_instr_def)
 qed
 
 
     
 lemma fits_first:
-  "[| 0 < length is; wtl_inst_list is G rT cert mxs (length is) 0 s \<noteq> Err; 
-      fits phi is G rT s mxs cert |] ==> 
+  "[| 0 < length is; wtl_inst_list is G rT cert mxs mxr (length is) et 0 s \<noteq> Err; 
+      fits phi is G rT s mxs mxr et cert |] ==> 
   G \<turnstile> s <=' phi ! 0"
 proof -
-  assume wtl:  "wtl_inst_list is G rT cert mxs (length is) 0 s \<noteq> Err"
-  assume fits: "fits phi is G rT s mxs cert"
+  assume wtl:  "wtl_inst_list is G rT cert mxs mxr (length is) et 0 s \<noteq> Err"
+  assume fits: "fits phi is G rT s mxs mxr et cert"
   assume pc:   "0 < length is"
 
   from wtl
-  have wt0: "wtl_inst_list (take 0 is) G rT cert mxs (length is) 0 s = OK s"
+  have wt0: "wtl_inst_list (take 0 is) G rT cert mxs mxr (length is) et 0 s = OK s"
     by simp
   
   with fits pc
@@ -244,11 +222,11 @@ proof -
     by (auto simp add: neq_Nil_conv)
   with wtl
   obtain s' where
-    "wtl_cert x G rT s cert mxs (length is) 0 = OK s'"
+    "wtl_cert x G rT s cert mxs mxr (length is) et 0 = OK s'"
     by auto
   hence 
     "!!t. cert!0 = Some t ==> G \<turnstile> s <=' cert!0"
-    by (simp add: wtl_cert_def split: if_splits)
+    by (simp add: wtl_cert_def split: split_if_asm)
 
   ultimately
   show ?thesis
@@ -257,18 +235,18 @@ qed
 
   
 lemma wtl_method_correct:
-"wtl_method G C pTs rT mxs mxl ins cert ==> \<exists> phi. wt_method G C pTs rT mxs mxl ins phi"
+"wtl_method G C pTs rT mxs mxl et ins cert ==> \<exists> phi. wt_method G C pTs rT mxs mxl ins et phi"
 proof (unfold wtl_method_def, simp only: Let_def, elim conjE)
   let "?s0" = "Some ([], OK (Class C) # map OK pTs @ replicate mxl Err)"
   assume pc:  "0 < length ins"
-  assume wtl: "wtl_inst_list ins G rT cert mxs (length ins) 0 ?s0 \<noteq> Err"
+  assume wtl: "wtl_inst_list ins G rT cert mxs mxl (length ins) et 0 ?s0 \<noteq> Err"
 
-  obtain phi where fits: "fits phi ins G rT ?s0 mxs cert"    
+  obtain phi where fits: "fits phi ins G rT ?s0 mxs mxl et cert"    
     by (rule exists_phi [elim_format]) blast
 
   with wtl
   have allpc:
-    "\<forall>pc. pc < length ins --> wt_instr (ins ! pc) G rT phi mxs (length ins) pc"
+    "\<forall>pc. pc < length ins --> wt_instr (ins ! pc) G rT phi mxs (length ins) et pc"
     by (blast intro: wtl_fits_wt)
 
   from pc wtl fits
@@ -285,8 +263,8 @@ theorem wtl_correct:
 proof -  
   assume wtl: "wtl_jvm_prog G cert"
 
-  let ?Phi = "\<lambda>C sig. let (C,rT,(maxs,maxl,ins)) = the (method (G,C) sig) in 
-              SOME phi. wt_method G C (snd sig) rT maxs maxl ins phi"
+  let ?Phi = "\<lambda>C sig. let (C,rT,(maxs,maxl,ins,et)) = the (method (G,C) sig) in 
+              SOME phi. wt_method G C (snd sig) rT maxs maxl ins et phi"
    
   { fix C S fs mdecls sig rT code
     assume "(C,S,fs,mdecls) \<in> set G" "(sig,rT,code) \<in> set mdecls"
