src/HOL/MicroJava/BV/LBVSpec.thy
@@ -6,186 +6,227 @@
 
 header {* The Lightweight Bytecode Verifier *}
 
+theory LBVSpec = Effect + Kildall:
 
-theory LBVSpec = Step :
+text {* 
+  The Lightweight Bytecode Verifier with exceptions has not 
+  made it completely into the Isabelle 2001 release. Currently 
+  there is only the specification itself available. The proofs of
+  soundness and completeness are broken (they still need to be
+  ported to the exception version). Both theories are included
+  for documentation (but they don't work for this specification), 
+  please see the Isabelle 99-2 release for a working copy.
+*}
 
 types
   certificate       = "state_type option list" 
   class_certificate = "sig => certificate"
   prog_certificate  = "cname => class_certificate"
 
+consts
+  merge :: "[jvm_prog, p_count, nat, nat, p_count, certificate, (nat \<times> (state_type option)) list, state] \<Rightarrow> state"
+primrec
+  "merge G pc mxs mxr max_pc cert []     x = x"
+  "merge G pc mxs mxr max_pc cert (s#ss) x = (let (pc',s') = s in 
+                                       if pc' < max_pc \<and> pc' = pc+1 then 
+                                         merge G pc mxs mxr max_pc cert ss (OK s' +_(sup G mxs mxr) x) 
+                                       else if pc' < max_pc \<and> G \<turnstile> s' <=' cert!pc' then 
+                                         merge G pc mxs mxr max_pc cert ss x
+                                       else Err)"
 
-constdefs
-  check_cert :: "[instr, jvm_prog, state_type option, certificate, p_count, p_count]
-                 => bool"
-  "check_cert i G s cert pc max_pc == \<forall>pc' \<in> set (succs i pc). pc' < max_pc \<and>  
-                                     (pc' \<noteq> pc+1 --> G \<turnstile> step i G s <=' cert!pc')"
-
-  wtl_inst :: "[instr,jvm_prog,ty,state_type option,certificate,nat,p_count,p_count] 
+constdefs 
+  wtl_inst :: "[instr,jvm_prog,ty,state_type option,certificate,nat,nat,p_count,exception_table,p_count] 
                => state_type option err" 
-  "wtl_inst i G rT s cert maxs max_pc pc == 
-     if app i G maxs rT s \<and> check_cert i G s cert pc max_pc then 
-       if pc+1 mem (succs i pc) then OK (step i G s) else OK (cert!(pc+1))
+  "wtl_inst i G rT s cert maxs maxr max_pc et pc == 
+     if app i G maxs rT pc et s then 
+       merge G pc maxs maxr max_pc cert (eff i G pc et s) (OK (cert!(pc+1)))
      else Err"
 
-constdefs
-  wtl_cert :: "[instr,jvm_prog,ty,state_type option,certificate,nat,p_count,p_count] 
+  wtl_cert :: "[instr,jvm_prog,ty,state_type option,certificate,nat,nat,p_count,exception_table,p_count] 
                => state_type option err"  
-  "wtl_cert i G rT s cert maxs max_pc pc ==
+  "wtl_cert i G rT s cert maxs maxr max_pc et pc ==
      case cert!pc of
-        None    => wtl_inst i G rT s cert maxs max_pc pc
+        None    => wtl_inst i G rT s cert maxs maxr max_pc et pc
       | Some s' => if G \<turnstile> s <=' (Some s') then 
-                    wtl_inst i G rT (Some s') cert maxs max_pc pc 
+                    wtl_inst i G rT (Some s') cert maxs maxr max_pc et pc 
                   else Err"
 
 consts 
-  wtl_inst_list :: "[instr list,jvm_prog,ty,certificate,nat,p_count,p_count, 
+  wtl_inst_list :: "[instr list,jvm_prog,ty,certificate,nat,nat,p_count,exception_table,p_count,
                      state_type option] => state_type option err"
 primrec
-  "wtl_inst_list []     G rT cert maxs max_pc pc s = OK s"
-  "wtl_inst_list (i#is) G rT cert maxs max_pc pc s = 
-    (let s' = wtl_cert i G rT s cert maxs max_pc pc in
-     strict (wtl_inst_list is G rT cert maxs max_pc (pc+1)) s')"
+  "wtl_inst_list []     G rT cert maxs maxr max_pc et pc s = OK s"
+  "wtl_inst_list (i#is) G rT cert maxs maxr max_pc et pc s = 
+    (let s' = wtl_cert i G rT s cert maxs maxr max_pc et pc in
+     strict (wtl_inst_list is G rT cert maxs maxr max_pc et (pc+1)) s')"
               
 
 constdefs
- wtl_method :: "[jvm_prog,cname,ty list,ty,nat,nat,instr list,certificate] => bool"  
- "wtl_method G C pTs rT mxs mxl ins cert ==  
+ wtl_method :: "[jvm_prog,cname,ty list,ty,nat,nat,exception_table,instr list,certificate] => bool"  
+ "wtl_method G C pTs rT mxs mxl et ins cert ==  
 	let max_pc = length ins  
   in 
   0 < max_pc \<and>   
-  wtl_inst_list ins G rT cert mxs max_pc 0 
+  wtl_inst_list ins G rT cert mxs mxl max_pc et 0 
                 (Some ([],(OK (Class C))#((map OK pTs))@(replicate mxl Err))) \<noteq> Err"
 
  wtl_jvm_prog :: "[jvm_prog,prog_certificate] => bool" 
  "wtl_jvm_prog G cert ==  
-  wf_prog (\<lambda>G C (sig,rT,maxs,maxl,b). wtl_method G C (snd sig) rT maxs maxl b (cert C sig)) G"
+  wf_prog (\<lambda>G C (sig,rT,maxs,maxl,b,et). wtl_method G C (snd sig) rT maxs maxl et b (cert C sig)) G"
 
 
 lemmas [iff] = not_Err_eq
 
+lemma if_eq_cases:
+  "(P \<Longrightarrow> x = z) \<Longrightarrow> (\<not>P \<Longrightarrow> y = z) \<Longrightarrow> (if P then x else y) = z"
+  by simp
+
+lemma merge_def:
+  "!!x. merge G pc mxs mxr max_pc cert ss x = 
+  (if \<forall>(pc',s') \<in> set ss. pc' < max_pc \<and> (pc' \<noteq> pc+1 \<longrightarrow> G \<turnstile> s' <=' cert!pc') then
+    map (OK \<circ> snd) [(p',t') \<in> ss. p'=pc+1] ++_(sup G mxs mxr) x
+  else Err)" (is "!!x. ?merge ss x = ?if ss x" is "!!x. ?P ss x")
+proof (induct ss)
+  show "!!x. ?P [] x" by simp
+next
+  have OK_snd: "(\<lambda>u. OK (snd u)) = OK \<circ> snd" by (rule ext) auto
+  fix x ss and s::"nat \<times> (state_type option)"
+  assume IH: "\<And>x. ?P ss x"
+  obtain pc' s' where s: "s = (pc',s')" by (cases s)  
+  hence "?merge (s#ss) x = ?merge ((pc',s')#ss) x" by hypsubst (rule refl)
+  also
+  have "\<dots> = (if pc' < max_pc \<and> pc' = pc+1 then 
+               ?merge ss (OK s' +_(sup G mxs mxr) x)
+             else if pc' < max_pc \<and> G \<turnstile> s' <=' cert!pc' then 
+               ?merge ss x
+             else Err)" 
+    (is "_ = (if ?pc' then ?merge ss (_ +_?f _) else if ?G then _ else _)")
+    by simp 
+  also 
+  let "if ?all ss then _ else _" = "?if ss x"    
+  have "\<dots> = ?if ((pc',s')#ss) x"
+  proof (cases "?pc'")    
+    case True
+    hence "?all (((pc',s')#ss)) = (pc+1 < max_pc \<and> ?all ss)" by simp
+    with True
+    have "?if ss (OK s' +_?f x) = ?if ((pc',s')#ss) x" by (auto simp add: OK_snd)
+    hence "?merge ss (OK s' +_?f x) = ?if ((pc',s')#ss) x" by (simp only: IH)
+    with True show ?thesis by (fast intro: if_eq_cases)
+  next
+    case False
+    have "(if ?G then ?merge ss x else Err) = ?if ((pc',s')#ss) x" 
+    proof (cases ?G)
+      assume G: ?G with False
+      have "?if ss x = ?if ((pc',s')#ss) x" by (auto simp add: OK_snd)
+      hence "?merge ss x = ?if ((pc',s')#ss) x" by (simp only: IH)
+      with G show ?thesis by (fast intro: if_eq_cases)
+    next
+      assume G: "\<not>?G"
+      with False have "Err = ?if ((pc',s')#ss) x" by auto
+      with G show ?thesis by (fast intro: if_eq_cases)
+    qed
+    with False show ?thesis by (fast intro: if_eq_cases)
+  qed
+  also from s have "\<dots> = ?if (s#ss) x" by hypsubst (rule refl)
+  finally show "?P (s#ss) x" .
+qed
+  
 
 lemma wtl_inst_OK:
-"(wtl_inst i G rT s cert maxs max_pc pc = OK s') =
- (app i G maxs rT s \<and> (\<forall>pc' \<in> set (succs i pc). 
-                       pc' < max_pc \<and> (pc' \<noteq> pc+1 --> G \<turnstile> step i G s <=' cert!pc')) \<and> 
- (if pc+1 \<in> set (succs i pc) then s' = step i G s else s' = cert!(pc+1)))"
-  by (auto simp add: wtl_inst_def check_cert_def set_mem_eq)
+"(wtl_inst i G rT s cert mxs mxr max_pc et pc = OK s') = (
+ app i G mxs rT pc et s \<and> 
+  (\<forall>(pc',r) \<in> set (eff i G pc et s). 
+  pc' < max_pc \<and> (pc' \<noteq> pc+1 \<longrightarrow> G \<turnstile> r <=' cert!pc')) \<and> 
+  map (OK \<circ> snd) [(p',t') \<in> (eff i G pc et s). p'=pc+1] 
+  ++_(sup G mxs mxr) (OK (cert!(pc+1))) = OK s')"
+  by (auto simp add: wtl_inst_def merge_def split: split_if_asm)
 
 lemma wtl_Cons:
-  "wtl_inst_list (i#is) G rT cert maxs max_pc pc s \<noteq> Err = 
-  (\<exists>s'. wtl_cert i G rT s cert maxs max_pc pc = OK s' \<and> 
-        wtl_inst_list is G rT cert maxs max_pc (pc+1) s' \<noteq> Err)"
+  "wtl_inst_list (i#is) G rT cert maxs maxr max_pc et pc s \<noteq> Err = 
+  (\<exists>s'. wtl_cert i G rT s cert maxs maxr max_pc et pc = OK s' \<and> 
+        wtl_inst_list is G rT cert maxs maxr max_pc et (pc+1) s' \<noteq> Err)"
   by (auto simp del: split_paired_Ex)
 
 lemma wtl_append:
-"\<forall> s pc. (wtl_inst_list (a@b) G rT cert mxs mpc pc s = OK s') =
-   (\<exists>s''. wtl_inst_list a G rT cert mxs mpc pc s = OK s'' \<and> 
-          wtl_inst_list b G rT cert mxs mpc (pc+length a) s'' = OK s')" 
+"\<forall> s pc. (wtl_inst_list (a@b) G rT cert mxs mxr mpc et pc s = OK s') =
+   (\<exists>s''. wtl_inst_list a G rT cert mxs mxr mpc et pc s = OK s'' \<and> 
+          wtl_inst_list b G rT cert mxs mxr mpc et (pc+length a) s'' = OK s')" 
   (is "\<forall> s pc. ?C s pc a" is "?P a")
 proof (induct ?P a)
-
   show "?P []" by simp
-  
-  fix x xs
-  assume IH: "?P xs"
-
+next
+  fix x xs  assume IH: "?P xs"
   show "?P (x#xs)"
   proof (intro allI)
     fix s pc 
-
     show "?C s pc (x#xs)"
-    proof (cases "wtl_cert x G rT s cert mxs mpc pc")
+    proof (cases "wtl_cert x G rT s cert mxs mxr mpc et pc")
       case Err thus ?thesis by simp
     next
-      fix s0
-      assume OK: "wtl_cert x G rT s cert mxs mpc pc = OK s0"
-
-      with IH
-      have "?C s0 (Suc pc) xs" by blast
-      
-      with OK
-      show ?thesis by simp
+      fix s0 assume "wtl_cert x G rT s cert mxs mxr mpc et pc = OK s0"      
+      with IH have "?C s0 (Suc pc) xs" by blast
+      thus ?thesis by (simp!)
     qed
   qed
 qed
 
 lemma wtl_take:
-  "wtl_inst_list is G rT cert mxs mpc pc s = OK s'' ==>
-   \<exists>s'. wtl_inst_list (take pc' is) G rT cert mxs mpc pc s = OK s'"
+  "wtl_inst_list is G rT cert mxs mxr mpc et pc s = OK s'' ==>
+   \<exists>s'. wtl_inst_list (take pc' is) G rT cert mxs mxr mpc et pc s = OK s'"
 proof -
-  assume "wtl_inst_list is G rT cert mxs mpc pc s = OK s''"
-
-  hence "wtl_inst_list (take pc' is @ drop pc' is) G rT cert mxs mpc pc s = OK s''"
+  assume "wtl_inst_list is G rT cert mxs mxr mpc et pc s = OK s''"
+  hence "wtl_inst_list (take pc' is @ drop pc' is) G rT cert mxs mxr mpc et pc s = OK s''"
     by simp
-
-  thus ?thesis 
-    by (auto simp add: wtl_append simp del: append_take_drop_id)
+  thus ?thesis by (auto simp add: wtl_append simp del: append_take_drop_id)
 qed
 
 lemma take_Suc:
   "\<forall>n. n < length l --> take (Suc n) l = (take n l)@[l!n]" (is "?P l")
 proof (induct l)
   show "?P []" by simp
-
-  fix x xs
-  assume IH: "?P xs"
-  
+next
+  fix x xs assume IH: "?P xs"  
   show "?P (x#xs)"
   proof (intro strip)
-    fix n
-    assume "n < length (x#xs)"
-    with IH
-    show "take (Suc n) (x # xs) = take n (x # xs) @ [(x # xs) ! n]"
-      by - (cases n, auto)
+    fix n assume "n < length (x#xs)"
+    with IH show "take (Suc n) (x # xs) = take n (x # xs) @ [(x # xs) ! n]" 
+      by (cases n, auto)
   qed
 qed
 
 lemma wtl_Suc:
- "[| wtl_inst_list (take pc is) G rT cert maxs (length is) 0 s = OK s'; 
-     wtl_cert (is!pc) G rT s' cert maxs (length is) pc = OK s'';
+ "[| wtl_inst_list (take pc is) G rT cert maxs maxr (length is) et 0 s = OK s'; 
+     wtl_cert (is!pc) G rT s' cert maxs maxr (length is) et pc = OK s'';
      Suc pc < length is |] ==>
-  wtl_inst_list (take (Suc pc) is) G rT cert maxs (length is) 0 s = OK s''" 
+  wtl_inst_list (take (Suc pc) is) G rT cert maxs maxr (length is) et 0 s = OK s''" 
 proof -
-  assume wtt: "wtl_inst_list (take pc is) G rT cert maxs (length is) 0 s = OK s'"
-  assume wtc: "wtl_cert (is!pc) G rT s' cert maxs (length is) pc = OK s''"
-  assume pc: "Suc pc < length is"
-
-  hence "take (Suc pc) is = (take pc is)@[is!pc]" 
-    by (simp add: take_Suc)
-
-  with wtt wtc pc
-  show ?thesis
-    by (simp add: wtl_append min_def)
+  assume "wtl_inst_list (take pc is) G rT cert maxs maxr (length is) et 0 s = OK s'"
+         "wtl_cert (is!pc) G rT s' cert maxs maxr (length is) et pc = OK s''"
+         "Suc pc < length is"
+  hence "take (Suc pc) is = (take pc is)@[is!pc]" by (simp add: take_Suc)
+  thus ?thesis by (simp! add: wtl_append min_def)
 qed
 
 lemma wtl_all:
-  "[| wtl_inst_list is G rT cert maxs (length is) 0 s \<noteq> Err;
+  "[| wtl_inst_list is G rT cert maxs maxr (length is) et 0 s \<noteq> Err;
       pc < length is |] ==> 
-   \<exists>s' s''. wtl_inst_list (take pc is) G rT cert maxs (length is) 0 s = OK s' \<and> 
-            wtl_cert (is!pc) G rT s' cert maxs (length is) pc = OK s''"
+   \<exists>s' s''. wtl_inst_list (take pc is) G rT cert maxs maxr (length is) et 0 s = OK s' \<and> 
+            wtl_cert (is!pc) G rT s' cert maxs maxr (length is) et pc = OK s''"
 proof -
-  assume all: "wtl_inst_list is G rT cert maxs (length is) 0 s \<noteq> Err"
+  assume all: "wtl_inst_list is G rT cert maxs maxr (length is) et 0 s \<noteq> Err"
 
   assume pc: "pc < length is"
   hence  "0 < length (drop pc is)" by simp
-  then 
-  obtain i r where 
-    Cons: "drop pc is = i#r" 
+  then  obtain i r where Cons: "drop pc is = i#r" 
     by (auto simp add: neq_Nil_conv simp del: length_drop)
   hence "i#r = drop pc is" ..
-  with all
-  have take: "wtl_inst_list (take pc is@i#r) G rT cert maxs (length is) 0 s \<noteq> Err"
+  with all have take: 
+    "wtl_inst_list (take pc is@i#r) G rT cert maxs maxr (length is) et 0 s \<noteq> Err"
     by simp
  
-  from pc
-  have "is!pc = drop pc is ! 0" by simp
-  with Cons
-  have "is!pc = i" by simp
-
-  with take pc
-  show ?thesis
-    by (auto simp add: wtl_append min_def)
+  from pc have "is!pc = drop pc is ! 0" by simp
+  with Cons have "is!pc = i" by simp
+  with take pc show ?thesis by (auto simp add: wtl_append min_def)
 qed
 
 
