src/HOL/MicroJava/BV/Typing_Framework.thy
@@ -11,29 +11,28 @@ theory Typing_Framework = Listn:
 text {* 
   The relationship between dataflow analysis and a welltyped-insruction predicate. 
 *}
+types
+  's step_type = "nat \<Rightarrow> 's \<Rightarrow> (nat \<times> 's) list"
 
 constdefs
- bounded :: "(nat => nat list) => nat => bool"
-"bounded succs n == !p<n. !q:set(succs p). q<n"
+ bounded :: "'s step_type => nat => bool"
+"bounded step n == !p<n. !s. !(q,t):set(step p s). q<n"  
 
- stable :: "'s ord =>
-           (nat => 's => 's)
-           => (nat => nat list) => 's list => nat => bool"
-"stable r step succs ss p == !q:set(succs p). step p (ss!p) <=_r ss!q"
+ stable :: "'s ord => 's step_type => 's list => nat => bool"
+"stable r step ss p == !(q,s'):set(step p (ss!p)). s' <=_r ss!q"
 
- stables :: "'s ord => (nat => 's => 's)
-            => (nat => nat list) => 's list => bool"
-"stables r step succs ss == !p<size ss. stable r step succs ss p"
+ stables :: "'s ord => 's step_type => 's list => bool"
+"stables r step ss == !p<size ss. stable r step ss p"
 
- is_bcv :: "'s ord => 's => (nat => 's => 's) => (nat => nat list)
-           => nat => 's set => ('s list => 's list) => bool"
-"is_bcv r T step succs n A bcv == !ss : list n A.
+ is_bcv :: "'s ord => 's => 's step_type 
+           => nat => 's set => ('s list => 's list) => bool"  
+"is_bcv r T step n A bcv == !ss : list n A.
    (!p<n. (bcv ss)!p ~= T) =
-   (? ts: list n A. ss <=[r] ts & wt_step r T step succs ts)"
+   (? ts: list n A. ss <=[r] ts & wt_step r T step ts)"
 
  wt_step ::
-"'s ord => 's => (nat => 's => 's) => (nat => nat list) => 's list => bool"
-"wt_step r T step succs ts ==
- !p<size(ts). ts!p ~= T & stable r step succs ts p"
+"'s ord => 's => 's step_type => 's list => bool"
+"wt_step r T step ts ==
+ !p<size(ts). ts!p ~= T & stable r step ts p"
 
 end
