src/HOL/MicroJava/BV/Typing_Framework_err.thy
@@ -11,134 +11,133 @@ theory Typing_Framework_err = Typing_Framework:
 
 constdefs
 
-dynamic_wt :: "'s ord => (nat => 's err => 's err) => (nat => nat list) => 
-               's err list => bool"
-"dynamic_wt r step succs ts == wt_step (Err.le r) Err step succs ts"
+dynamic_wt :: "'s ord => 's err step_type => 's err list => bool"
+"dynamic_wt r step ts == wt_step (Err.le r) Err step ts"
 
-static_wt :: "'s ord => (nat => 's => bool) => 
-              (nat => 's => 's) => (nat => nat list) =>  's list => bool"
-"static_wt r app step succs ts == 
-  !p < size ts. app p (ts!p) & (!q:set(succs p). step p (ts!p) <=_r ts!q)"
+static_wt :: "'s ord => (nat => 's => bool) => 's step_type => 's list => bool"
+"static_wt r app step ts == 
+  \<forall>p < size ts. app p (ts!p) \<and> (\<forall>(q,t) \<in> set (step p (ts!p)). t <=_r ts!q)"
 
-err_step :: "(nat => 's => bool) => (nat => 's => 's) => 
-             (nat => 's err => 's err)"
-"err_step app step p == lift (%t. if app p t then OK (step p t) else Err)"
+map_snd :: "('b \<Rightarrow> 'c) \<Rightarrow> ('a \<times> 'b) list \<Rightarrow> ('a \<times> 'c) list"
+"map_snd f == map (\<lambda>(x,y). (x, f y))"
 
-non_empty :: "(nat => nat list) => bool"
-"non_empty succs == !p. succs p ~= []"
+map_err :: "('a \<times> 'b) list \<Rightarrow> ('a \<times> 'b err) list"
+"map_err == map_snd (\<lambda>y. Err)"
 
+err_step :: "(nat \<Rightarrow> 's \<Rightarrow> bool) \<Rightarrow> 's step_type \<Rightarrow> 's err step_type"
+"err_step app step p t == case t of Err \<Rightarrow> map_err (step p arbitrary) | OK t' \<Rightarrow> 
+  if app p t' then map_snd OK (step p t') else map_err (step p t')"
+
+non_empty :: "'s step_type => bool"
+"non_empty step == \<forall>p t. step p t \<noteq> []"
+
+
+lemmas err_step_defs = err_step_def map_snd_def map_err_def
 
 lemma non_emptyD:
-  "non_empty succs ==> ? q. q:set(succs p)"
+  "non_empty step ==> \<exists>q t'. (q,t') \<in> set(step p t)"
 proof (unfold non_empty_def)
-  assume "!p. succs p ~= []"
-  hence "succs p ~= []" ..
-  then obtain x xs where "succs p = x#xs"
+  assume "\<forall>p t. step p t \<noteq> []"
+  hence "step p t \<noteq> []" by blast
+  then obtain x xs where "step p t = x#xs"
     by (auto simp add: neq_Nil_conv)
-  thus ?thesis 
-    by auto
+  hence "x \<in> set(step p t)" by simp
+  thus ?thesis by (cases x) blast
 qed
 
+
 lemma dynamic_imp_static:
-  "[| bounded succs (size ts); non_empty succs;
-      dynamic_wt r (err_step app step) succs ts |] 
-  ==> static_wt r app step succs (map ok_val ts)"
+  "[| bounded step (size ts); non_empty step;
+      dynamic_wt r (err_step app step) ts |] 
+  ==> static_wt r app step (map ok_val ts)"
 proof (unfold static_wt_def, intro strip, rule conjI)
 
-  assume b:  "bounded succs (size ts)"
-  assume n:  "non_empty succs"
-  assume wt: "dynamic_wt r (err_step app step) succs ts"
+  assume b:  "bounded step (size ts)"
+  assume n:  "non_empty step"
+  assume wt: "dynamic_wt r (err_step app step) ts"
 
   fix p 
   assume "p < length (map ok_val ts)"
   hence lp: "p < length ts" by simp
 
   from wt lp
-  have [intro?]: "!!p. p < length ts ==> ts ! p ~= Err" 
+  have [intro?]: "\<And>p. p < length ts \<Longrightarrow> ts ! p \<noteq> Err" 
     by (unfold dynamic_wt_def wt_step_def) simp
 
   show app: "app p (map ok_val ts ! p)"
   proof -
-    from n
-    obtain q where q: "q:set(succs p)"
-      by (auto dest: non_emptyD)
-
-    from wt lp q
+    from wt lp 
     obtain s where
       OKp:  "ts ! p = OK s" and
-      less: "err_step app step p (ts ! p) <=_(Err.le r) ts ! q"
+      less: "\<forall>(q,t) \<in> set (err_step app step p (ts!p)). t <=_(Err.le r) ts!q"
       by (unfold dynamic_wt_def wt_step_def stable_def) 
          (auto iff: not_Err_eq)
+    
+    from n
+    obtain q t where q: "(q,t) \<in> set(step p s)"
+      by (blast dest: non_emptyD)
 
     from lp b q
-    have lq: "q < length ts"
-      by (unfold bounded_def) blast
-    hence "ts!q ~= Err" ..
-    then
-    obtain s' where OKq: "ts ! q = OK s'"
-      by (auto iff: not_Err_eq)      
+    have lq: "q < length ts" by (unfold bounded_def) blast
+    hence "ts!q \<noteq> Err" ..
+    then obtain s' where OKq: "ts ! q = OK s'" by (auto iff: not_Err_eq)      
 
-    with OKp less
-    have "app p s"
-      by (simp add: err_step_def lift_def split: err.split_asm split_if_asm)
+    with OKp less q have "app p s"
+      by (auto simp add: err_step_defs split: err.split_asm split_if_asm)
 
-    with lp OKp
-    show ?thesis
-      by simp
+    with lp OKp show ?thesis by simp
   qed
   
-  show "!q:set(succs p). step p (map ok_val ts ! p) <=_r map ok_val ts ! q"
-  proof (intro strip)
-    fix q
-    assume q: "q:set (succs p)"
+  show "\<forall>(q,t)\<in>set(step p (map ok_val ts ! p)). t <=_r map ok_val ts ! q" 
+  proof clarify
+    fix q t assume q: "(q,t) \<in> set (step p (map ok_val ts ! p))"
 
     from wt lp q
     obtain s where
       OKp:  "ts ! p = OK s" and
-      less: "err_step app step p (ts ! p) <=_(Err.le r) ts ! q"
+      less: "\<forall>(q,t) \<in> set (err_step app step p (ts!p)). t <=_(Err.le r) ts!q"
       by (unfold dynamic_wt_def wt_step_def stable_def) 
          (auto iff: not_Err_eq)
 
     from lp b q
-    have lq: "q < length ts"
-      by (unfold bounded_def) blast
-    hence "ts!q ~= Err" ..
-    then
-    obtain s' where OKq: "ts ! q = OK s'"
-      by (auto iff: not_Err_eq)      
+    have lq: "q < length ts" by (unfold bounded_def) blast
+    hence "ts!q \<noteq> Err" ..
+    then obtain s' where OKq: "ts ! q = OK s'" by (auto iff: not_Err_eq)
 
-    from lp lq OKp OKq app less
-    show "step p (map ok_val ts ! p) <=_r map ok_val ts ! q"
-      by (simp add: err_step_def lift_def)
+    from lp lq OKp OKq app less q
+    show "t <=_r map ok_val ts ! q"
+      by (auto simp add: err_step_def map_snd_def) 
   qed
 qed
 
 
 lemma static_imp_dynamic:
-  "[| static_wt r app step succs ts; bounded succs (size ts) |] 
-  ==> dynamic_wt r (err_step app step) succs (map OK ts)"
+  "[| static_wt r app step ts; bounded step (size ts) |] 
+  ==> dynamic_wt r (err_step app step) (map OK ts)"
 proof (unfold dynamic_wt_def wt_step_def, intro strip, rule conjI)
-  assume bounded: "bounded succs (size ts)"
-  assume static:  "static_wt r app step succs ts"
+  assume bounded: "bounded step (size ts)"
+  assume static:  "static_wt r app step ts"
   fix p assume "p < length (map OK ts)" 
   hence p: "p < length ts" by simp
   thus "map OK ts ! p \<noteq> Err" by simp
-  { fix q
-    assume q: "q : set (succs p)"
+  { fix q t
+    assume q: "(q,t) \<in> set (err_step app step p (map OK ts ! p))" 
     with p static obtain 
-      "app p (ts ! p)" "step p (ts ! p) <=_r ts ! q"
+      "app p (ts ! p)" "\<forall>(q,t) \<in> set (step p (ts!p)). t <=_r ts!q"
       by (unfold static_wt_def) blast
     moreover
-    from q p bounded
-    have "q < size ts" by (unfold bounded_def) blast
+    from q p bounded have "q < size ts" 
+      by (clarsimp simp add: bounded_def err_step_defs 
+          split: err.splits split_if_asm) blast+
     hence "map OK ts ! q = OK (ts!q)" by simp
     moreover
     have "p < size ts" by (rule p)
+    moreover note q
     ultimately     
-    have "err_step app step p (map OK ts ! p) <=_(Err.le r) map OK ts ! q"
-      by (simp add: err_step_def lift_def)
+    have "t <=_(Err.le r) map OK ts ! q" 
+      by (auto simp add: err_step_def map_snd_def)
   }
-  thus "stable (Err.le r) (err_step app step) succs (map OK ts) p"
+  thus "stable (Err.le r) (err_step app step) (map OK ts) p"
     by (unfold stable_def) blast
 qed
 
